hs-to-coq/examples/ghc-base/manual/Data/Foldable.v
@@ -25,8 +25,6 @@ Require GHC.Generics.
 Require GHC.Num.
 (* Require #. *)
 Require Coq.Program.Basics.
-Require GHC.BaseGen.
-Require GHC.Prim.
 Require GHC.Tuple.
 Require GHC.Types.
 
@@ -36,7 +34,7 @@ Definition one  : BinNums.Z := BinNums.Zpos BinNums.xH.
 (*
 Definition hashDotop___ {b} {c} {a} `{GHC.Types.Coercible b c}
     : (b -> c) -> (a -> b) -> (a -> c) :=
-  fun arg_76__ => match arg_76__ with | _f => GHC.Prim.coerce end.
+  fun arg_76__ => match arg_76__ with | _f => GHC.Base.coerce end.
 
 Infix "hashDot" := (hashDotop___) (at level 99).
 
@@ -65,7 +63,7 @@ Local Definition instance_Foldable_option_foldl1 : forall {a},
                         match arg_46__ , arg_47__ with
                           | m , y => Some (match m with | None => y | (Some x) => f x y end)
                         end in
-                    Data.Maybe.fromMaybe (GHC.Prim.errorWithoutStackTrace
+                    Data.Maybe.fromMaybe (GHC.Base.errorWithoutStackTrace
                                          &"foldl1: empty structure") (instance_Foldable_option_foldl mf None xs)
       end. *)
 
@@ -77,9 +75,9 @@ Local Definition instance_Foldable_option_foldr' : forall {a} {b},
         | f , z0 , xs => let f' :=
                            fun arg_12__ arg_13__ arg_14__ =>
                              match arg_12__ , arg_13__ , arg_14__ with
-                               | k , x , z => GHC.BaseGen.op_zdzn__ k (f x z)
+                               | k , x , z => GHC.Base.op_zdzn__ k (f x z)
                              end in
-                         instance_Foldable_option_foldl f' GHC.BaseGen.id xs z0
+                         instance_Foldable_option_foldl f' GHC.Base.id xs z0
       end.
 
 Local Definition instance_Foldable_option_foldr : forall {a} {b},
@@ -102,7 +100,7 @@ Local Definition instance_Foldable_option_foldr1 : forall {a},
                         match arg_36__ , arg_37__ with
                           | x , m => Some (match m with | None => x | (Some y) => f x y end)
                         end in
-                    Data.Maybe.fromMaybe (GHC.Prim.errorWithoutStackTrace
+                    Data.Maybe.fromMaybe (GHC.Base.errorWithoutStackTrace
                                          &"foldr1: empty structure") (instance_Foldable_option_foldr mf None xs)
       end.
 *)
@@ -115,7 +113,7 @@ Local Definition instance_Foldable_option_toList : forall {a},
   fun {a} =>
     fun arg_54__ =>
       match arg_54__ with
-        | t => Prim.build (fun _ arg_55__ arg_56__ =>
+        | t => Base.build (fun _ arg_55__ arg_56__ =>
                                 match arg_55__ , arg_56__ with
                                   | c , n => instance_Foldable_option_foldr c n t
                                 end)
@@ -129,9 +127,9 @@ Local Definition instance_Foldable_option_foldl' : forall {b} {a},
         | f , z0 , xs => let f' :=
                            fun arg_27__ arg_28__ arg_29__ =>
                              match arg_27__ , arg_28__ , arg_29__ with
-                               | x , k , z => GHC.BaseGen.op_zdzn__ k (f z x)
+                               | x , k , z => GHC.Base.op_zdzn__ k (f z x)
                              end in
-                         instance_Foldable_option_foldr f' GHC.BaseGen.id xs z0
+                         instance_Foldable_option_foldr f' GHC.Base.id xs z0
       end.
 
 Local Definition instance_Foldable_option_length : forall {a},
@@ -143,12 +141,12 @@ Local Definition instance_Foldable_option_length : forall {a},
                                       end) zero.
 
 Local Definition instance_Foldable_option_foldMap : forall {m} {a},
-                                                      forall `{GHC.BaseGen.Monoid m}, (a -> m) -> option a -> m :=
-  fun {m} {a} `{GHC.BaseGen.Monoid m} =>
+                                                      forall `{GHC.Base.Monoid m}, (a -> m) -> option a -> m :=
+  fun {m} {a} `{GHC.Base.Monoid m} =>
     fun arg_1__ =>
       match arg_1__ with
         | f => instance_Foldable_option_foldr (Coq.Program.Basics.compose
-                                              GHC.BaseGen.mappend f) GHC.BaseGen.mempty
+                                              GHC.Base.mappend f) GHC.Base.mempty
       end.
 (*
 Local Definition instance_Foldable_option_product : forall {a},
@@ -162,17 +160,17 @@ Local Definition instance_Foldable_option_sum : forall {a},
     hashDot getSum (instance_Foldable_option_foldMap Data.Monoid.Sum).
 *)
 Local Definition instance_Foldable_option_fold : forall {m},
-                                                   forall `{GHC.BaseGen.Monoid m}, option m -> m :=
-  fun {m} `{GHC.BaseGen.Monoid m} =>
-    instance_Foldable_option_foldMap GHC.BaseGen.id.
+                                                   forall `{GHC.Base.Monoid m}, option m -> m :=
+  fun {m} `{GHC.Base.Monoid m} =>
+    instance_Foldable_option_foldMap GHC.Base.id.
 
 Local Definition instance_Foldable_list_elem : forall {a},
-                                                 forall `{GHC.Prim.Eq_ a}, a -> list a -> bool :=
-  fun {a} `{GHC.Prim.Eq_ a} => GHC.List.elem.
+                                                 forall `{GHC.Base.Eq_ a}, a -> list a -> bool :=
+  fun {a} `{GHC.Base.Eq_ a} => GHC.List.elem.
 
 Local Definition instance_Foldable_list_foldl : forall {b} {a},
                                                   (b -> a -> b) -> b -> list a -> b :=
-  fun {b} {a} => Prim.foldl.
+  fun {b} {a} => Base.foldl.
 
 Local Definition instance_Foldable_list_foldr' : forall {a} {b},
                                                    (a -> b -> b) -> b -> list a -> b :=
@@ -182,14 +180,14 @@ Local Definition instance_Foldable_list_foldr' : forall {a} {b},
         | f , z0 , xs => let f' :=
                            fun arg_12__ arg_13__ arg_14__ =>
                              match arg_12__ , arg_13__ , arg_14__ with
-                               | k , x , z => GHC.BaseGen.op_zdzn__ k (f x z)
+                               | k , x , z => GHC.Base.op_zdzn__ k (f x z)
                              end in
-                         instance_Foldable_list_foldl f' GHC.BaseGen.id xs z0
+                         instance_Foldable_list_foldl f' GHC.Base.id xs z0
       end.
 
 Local Definition instance_Foldable_list_foldl' : forall {b} {a},
                                                    (b -> a -> b) -> b -> list a -> b :=
-  fun {b} {a} => Prim.foldl'.
+  fun {b} {a} => Base.foldl'.
 
 Local Definition instance_Foldable_list_foldl1 : forall {a},
                                                    (a -> a -> a) -> list a -> a :=
@@ -197,21 +195,21 @@ Local Definition instance_Foldable_list_foldl1 : forall {a},
 
 Local Definition instance_Foldable_list_foldr : forall {a} {b},
                                                   (a -> b -> b) -> b -> list a -> b :=
-  fun {a} {b} => GHC.BaseGen.foldr.
+  fun {a} {b} => GHC.Base.foldr.
 
 Local Definition instance_Foldable_list_foldMap : forall {m} {a},
-                                                    forall `{GHC.BaseGen.Monoid m}, (a -> m) -> list a -> m :=
-  fun {m} {a} `{GHC.BaseGen.Monoid m} =>
+                                                    forall `{GHC.Base.Monoid m}, (a -> m) -> list a -> m :=
+  fun {m} {a} `{GHC.Base.Monoid m} =>
     fun arg_1__ =>
       match arg_1__ with
-        | f => instance_Foldable_list_foldr (Coq.Program.Basics.compose GHC.BaseGen.mappend
-                                                                        f) GHC.BaseGen.mempty
+        | f => instance_Foldable_list_foldr (Coq.Program.Basics.compose GHC.Base.mappend
+                                                                        f) GHC.Base.mempty
       end.
 
 Local Definition instance_Foldable_list_fold : forall {m},
-                                                 forall `{GHC.BaseGen.Monoid m}, list m -> m :=
-  fun {m} `{GHC.BaseGen.Monoid m} =>
-    instance_Foldable_list_foldMap GHC.BaseGen.id.
+                                                 forall `{GHC.Base.Monoid m}, list m -> m :=
+  fun {m} `{GHC.Base.Monoid m} =>
+    instance_Foldable_list_foldMap GHC.Base.id.
 
 Local Definition instance_Foldable_list_foldr1 : forall {a},
                                                    (a -> a -> a) -> list a -> a :=
@@ -222,12 +220,12 @@ Local Definition instance_Foldable_list_length : forall {a},
   fun {a} => GHC.List.length.
 
 Local Definition instance_Foldable_list_maximum : forall {a},
-                                                    forall `{GHC.Prim.Ord a}, list a -> a :=
-  fun {a} `{GHC.Prim.Ord a} => GHC.List.maximum.
+                                                    forall `{GHC.Base.Ord a}, list a -> a :=
+  fun {a} `{GHC.Base.Ord a} => GHC.List.maximum.
 
 Local Definition instance_Foldable_list_minimum : forall {a},
-                                                    forall `{GHC.Prim.Ord a}, list a -> a :=
-  fun {a} `{GHC.Prim.Ord a} => GHC.List.minimum.
+                                                    forall `{GHC.Base.Ord a}, list a -> a :=
+  fun {a} `{GHC.Base.Ord a} => GHC.List.minimum.
 
 Local Definition instance_Foldable_list_null : forall {a}, list a -> bool :=
   fun {a} => GHC.List.null.
@@ -241,13 +239,13 @@ Local Definition instance_Foldable_list_sum : forall {a},
   fun {a} `{GHC.Num.Num a} => GHC.List.sum.
 
 Local Definition instance_Foldable_list_toList : forall {a}, list a -> list a :=
-  fun {a} => GHC.BaseGen.id.
+  fun {a} => GHC.Base.id.
 
 (*
 Local Definition instance_Foldable__GHC_Tuple_____a__foldMap : forall {m} {a},
-                                                                 forall `{GHC.BaseGen.Monoid m},
+                                                                 forall `{GHC.Base.Monoid m},
                                                                    (a -> m) -> (a * a) -> m :=
-  fun {m} {a} `{GHC.BaseGen.Monoid m} =>
+  fun {m} {a} `{GHC.Base.Monoid m} =>
     fun arg_286__ arg_287__ =>
       match arg_286__ , arg_287__ with
         | f , (pair _ y) => f y
@@ -261,7 +259,7 @@ Local Definition instance_Foldable__GHC_Tuple_____a__foldl : forall {b} {a},
       match arg_19__ , arg_20__ , arg_21__ with
         | f , z , t => Data.Monoid.appEndo (Data.Monoid.getDual (instance_Foldable__GHC_Tuple_____a__foldMap
                                         (Coq.Program.Basics.compose Data.Monoid.Dual (Coq.Program.Basics.compose
-                                                                    Data.Monoid.Endo (GHC.BaseGen.flip f))) t)) z
+                                                                    Data.Monoid.Endo (GHC.Base.flip f))) t)) z
       end.
 
 Local Definition instance_Foldable__GHC_Tuple_____a__foldl1 : forall {a},
@@ -274,7 +272,7 @@ Local Definition instance_Foldable__GHC_Tuple_____a__foldl1 : forall {a},
                         match arg_46__ , arg_47__ with
                           | m , y => Some (match m with | None => y | (Some x) => f x y end)
                         end in
-                    Data.Maybe.fromMaybe (GHC.Prim.errorWithoutStackTrace
+                    Data.Maybe.fromMaybe (GHC.Base.errorWithoutStackTrace
                                          &"foldl1: empty structure") (instance_Foldable__GHC_Tuple_____a__foldl mf None
                                                                      xs)
       end.
@@ -289,7 +287,7 @@ Local Definition instance_Foldable__GHC_Tuple_____a__foldr' : forall {a} {b},
                              match arg_12__ , arg_13__ , arg_14__ with
                                | k , x , z => GHC.Base.op_zdzn__ k (f x z)
                              end in
-                         instance_Foldable__GHC_Tuple_____a__foldl f' GHC.BaseGen.id xs z0
+                         instance_Foldable__GHC_Tuple_____a__foldl f' GHC.Base.id xs z0
       end.
 
 Local Definition instance_Foldable__GHC_Tuple_____a__product : forall {a},
@@ -321,7 +319,7 @@ Local Definition instance_Foldable__GHC_Tuple_____a__foldr1 : forall {a},
                         match arg_36__ , arg_37__ with
                           | x , m => Some (match m with | None => x | (Some y) => f x y end)
                         end in
-                    Data.Maybe.fromMaybe (GHC.Prim.errorWithoutStackTrace
+                    Data.Maybe.fromMaybe (GHC.Base.errorWithoutStackTrace
                                          &"foldr1: empty structure") (instance_Foldable__GHC_Tuple_____a__foldr mf None
                                                                      xs)
       end.
@@ -336,7 +334,7 @@ Local Definition instance_Foldable__GHC_Tuple_____a__toList : forall {a},
   fun {a} =>
     fun arg_54__ =>
       match arg_54__ with
-        | t => Prim.build (fun arg_55__ arg_56__ =>
+        | t => Base.build (fun arg_55__ arg_56__ =>
                                 match arg_55__ , arg_56__ with
                                   | c , n => instance_Foldable__GHC_Tuple_____a__foldr c n t
                                 end)
@@ -352,7 +350,7 @@ Local Definition instance_Foldable__GHC_Tuple_____a__foldl' : forall {b} {a},
                              match arg_27__ , arg_28__ , arg_29__ with
                                | x , k , z => GHC.Base.op_zdzn__ k (f z x)
                              end in
-                         instance_Foldable__GHC_Tuple_____a__foldr f' GHC.BaseGen.id xs z0
+                         instance_Foldable__GHC_Tuple_____a__foldr f' GHC.Base.id xs z0
       end.
 
 Local Definition instance_Foldable__GHC_Tuple_____a__length : forall {a},
@@ -380,9 +378,9 @@ Local Definition instance_Foldable__GHC_Arr_Array_i__foldr : forall {a} {b},
   fun {a} {b} => GHC.Arr.foldrElems.
 
 Local Definition instance_Foldable__GHC_Arr_Array_i__foldMap : forall {m} {a},
-                                                                 forall `{GHC.BaseGen.Monoid m},
+                                                                 forall `{GHC.Base.Monoid m},
                                                                    (a -> m) -> (GHC.Arr.Array i) a -> m :=
-  fun {m} {a} `{GHC.BaseGen.Monoid m} =>
+  fun {m} {a} `{GHC.Base.Monoid m} =>
     fun arg_1__ =>
       match arg_1__ with
         | f => instance_Foldable__GHC_Arr_Array_i__foldr (Coq.Program.Basics.compose
@@ -401,10 +399,10 @@ Local Definition instance_Foldable__GHC_Arr_Array_i__sum : forall {a},
     hashDot getSum (instance_Foldable__GHC_Arr_Array_i__foldMap Data.Monoid.Sum).
 
 Local Definition instance_Foldable__GHC_Arr_Array_i__fold : forall {m},
-                                                              forall `{GHC.BaseGen.Monoid m},
+                                                              forall `{GHC.Base.Monoid m},
                                                                 (GHC.Arr.Array i) m -> m :=
-  fun {m} `{GHC.BaseGen.Monoid m} =>
-    instance_Foldable__GHC_Arr_Array_i__foldMap GHC.BaseGen.id.
+  fun {m} `{GHC.Base.Monoid m} =>
+    instance_Foldable__GHC_Arr_Array_i__foldMap GHC.Base.id.
 
 Local Definition instance_Foldable__GHC_Arr_Array_i__foldr' : forall {a} {b},
                                                                 (a -> b -> b) -> b -> (GHC.Arr.Array i) a -> b :=
@@ -423,7 +421,7 @@ Local Definition instance_Foldable__GHC_Arr_Array_i__null : forall {a},
   fun {a} =>
     fun arg_283__ =>
       match arg_283__ with
-        | a => GHC.Prim.op_zeze__ (GHC.Arr.numElements a) #0
+        | a => GHC.Base.op_zeze__ (GHC.Arr.numElements a) #0
       end.
 
 Local Definition instance_Foldable__GHC_Arr_Array_i__toList : forall {a},
@@ -432,19 +430,19 @@ Local Definition instance_Foldable__GHC_Arr_Array_i__toList : forall {a},
 *)
 
 Local Definition instance_Foldable_Data_Proxy_Proxy_elem : forall {a},
-                                                             forall `{GHC.Prim.Eq_ a},
+                                                             forall `{GHC.Base.Eq_ a},
                                                                a -> Data.Proxy.Proxy a -> bool :=
-  fun {a} `{GHC.Prim.Eq_ a} => fun arg_275__ arg_276__ => false.
+  fun {a} `{GHC.Base.Eq_ a} => fun arg_275__ arg_276__ => false.
 
 Local Definition instance_Foldable_Data_Proxy_Proxy_fold : forall {m},
-                                                             forall `{GHC.BaseGen.Monoid m}, Data.Proxy.Proxy m -> m :=
-  fun {m} `{GHC.BaseGen.Monoid m} => fun arg_254__ => GHC.BaseGen.mempty.
+                                                             forall `{GHC.Base.Monoid m}, Data.Proxy.Proxy m -> m :=
+  fun {m} `{GHC.Base.Monoid m} => fun arg_254__ => GHC.Base.mempty.
 
 Local Definition instance_Foldable_Data_Proxy_Proxy_foldMap : forall {m} {a},
-                                                                forall `{GHC.BaseGen.Monoid m},
+                                                                forall `{GHC.Base.Monoid m},
                                                                   (a -> m) -> Data.Proxy.Proxy a -> m :=
-  fun {m} {a} `{GHC.BaseGen.Monoid m} =>
-    fun arg_252__ arg_253__ => GHC.BaseGen.mempty.
+  fun {m} {a} `{GHC.Base.Monoid m} =>
+    fun arg_252__ arg_253__ => GHC.Base.mempty.
 
 Local Definition instance_Foldable_Data_Proxy_Proxy_foldl : forall {b} {a},
                                                               (b -> a -> b) -> b -> Data.Proxy.Proxy a -> b :=
@@ -462,16 +460,16 @@ Local Definition instance_Foldable_Data_Proxy_Proxy_foldr' : forall {a} {b},
         | f , z0 , xs => let f' :=
                            fun arg_12__ arg_13__ arg_14__ =>
                              match arg_12__ , arg_13__ , arg_14__ with
-                               | k , x , z => GHC.BaseGen.op_zdzn__ k (f x z)
+                               | k , x , z => GHC.Base.op_zdzn__ k (f x z)
                              end in
-                         instance_Foldable_Data_Proxy_Proxy_foldl f' GHC.BaseGen.id xs z0
+                         instance_Foldable_Data_Proxy_Proxy_foldl f' GHC.Base.id xs z0
       end.
 
 (*
 Local Definition instance_Foldable_Data_Proxy_Proxy_foldl1 : forall {a},
                                                                (a -> a -> a) -> Data.Proxy.Proxy a -> a :=
   fun {a} =>
-    fun arg_263__ arg_264__ => GHC.Prim.errorWithoutStackTrace &"foldl1: Proxy".
+    fun arg_263__ arg_264__ => GHC.Base.errorWithoutStackTrace &"foldl1: Proxy".
 *)
 Local Definition instance_Foldable_Data_Proxy_Proxy_foldr : forall {a} {b},
                                                               (a -> b -> b) -> b -> Data.Proxy.Proxy a -> b :=
@@ -486,7 +484,7 @@ Local Definition instance_Foldable_Data_Proxy_Proxy_toList : forall {a},
   fun {a} =>
     fun arg_54__ =>
       match arg_54__ with
-        | t => Prim.build (fun _ arg_55__ arg_56__ =>
+        | t => Base.build (fun _ arg_55__ arg_56__ =>
                                 match arg_55__ , arg_56__ with
                                   | c , n => instance_Foldable_Data_Proxy_Proxy_foldr c n t
                                 end)
@@ -500,16 +498,16 @@ Local Definition instance_Foldable_Data_Proxy_Proxy_foldl' : forall {b} {a},
         | f , z0 , xs => let f' :=
                            fun arg_27__ arg_28__ arg_29__ =>
                              match arg_27__ , arg_28__ , arg_29__ with
-                               | x , k , z => GHC.BaseGen.op_zdzn__ k (f z x)
+                               | x , k , z => GHC.Base.op_zdzn__ k (f z x)
                              end in
-                         instance_Foldable_Data_Proxy_Proxy_foldr f' GHC.BaseGen.id xs z0
+                         instance_Foldable_Data_Proxy_Proxy_foldr f' GHC.Base.id xs z0
       end.
 
 (*
 Local Definition instance_Foldable_Data_Proxy_Proxy_foldr1 : forall {a},
                                                                (a -> a -> a) -> Data.Proxy.Proxy a -> a :=
   fun {a} =>
-    fun arg_267__ arg_268__ => GHC.Prim.errorWithoutStackTrace &"foldr1: Proxy".
+    fun arg_267__ arg_268__ => GHC.Base.errorWithoutStackTrace &"foldr1: Proxy".
 *)
 Local Definition instance_Foldable_Data_Proxy_Proxy_length : forall {a},
                                                                Data.Proxy.Proxy a -> GHC.Num.Int :=
@@ -529,29 +527,29 @@ Local Definition instance_Foldable_Data_Proxy_Proxy_sum : forall {a},
 
 (*
 Local Definition instance_Foldable_Data_Monoid_Dual_elem : forall {a},
-                                                             forall `{GHC.Prim.Eq_ a},
+                                                             forall `{GHC.Base.Eq_ a},
                                                                a -> Data.Monoid.Dual a -> bool :=
-  fun {a} `{GHC.Prim.Eq_ a} =>
+  fun {a} `{GHC.Base.Eq_ a} =>
     hashDot (fun arg_236__ => Coq.Program.Basics.compose arg_236__ getDual)
-            GHC.Prim.op_zeze__.
+            GHC.Base.op_zeze__.
 
 Local Definition instance_Foldable_Data_Monoid_Dual_foldMap : forall {m} {a},
-                                                                forall `{GHC.BaseGen.Monoid m},
+                                                                forall `{GHC.Base.Monoid m},
                                                                   (a -> m) -> Data.Monoid.Dual a -> m :=
-  fun {m} {a} `{GHC.BaseGen.Monoid m} => GHC.Prim.coerce.
+  fun {m} {a} `{GHC.Base.Monoid m} => GHC.Base.coerce.
 
 Local Definition instance_Foldable_Data_Monoid_Dual_fold : forall {m},
-                                                             forall `{GHC.BaseGen.Monoid m}, Data.Monoid.Dual m -> m :=
-  fun {m} `{GHC.BaseGen.Monoid m} =>
-    instance_Foldable_Data_Monoid_Dual_foldMap GHC.BaseGen.id.
+                                                             forall `{GHC.Base.Monoid m}, Data.Monoid.Dual m -> m :=
+  fun {m} `{GHC.Base.Monoid m} =>
+    instance_Foldable_Data_Monoid_Dual_foldMap GHC.Base.id.
 
 Local Definition instance_Foldable_Data_Monoid_Dual_foldl : forall {b} {a},
                                                               (b -> a -> b) -> b -> Data.Monoid.Dual a -> b :=
-  fun {b} {a} => GHC.Prim.coerce.
+  fun {b} {a} => GHC.Base.coerce.
 
 Local Definition instance_Foldable_Data_Monoid_Dual_foldl' : forall {b} {a},
                                                                (b -> a -> b) -> b -> Data.Monoid.Dual a -> b :=
-  fun {b} {a} => GHC.Prim.coerce.
+  fun {b} {a} => GHC.Base.coerce.
 
 Local Definition instance_Foldable_Data_Monoid_Dual_foldl1 : forall {a},
                                                                (a -> a -> a) -> Data.Monoid.Dual a -> a :=
@@ -578,12 +576,12 @@ Local Definition instance_Foldable_Data_Monoid_Dual_length : forall {a},
   fun {a} => fun arg_245__ => one.
 
 Local Definition instance_Foldable_Data_Monoid_Dual_maximum : forall {a},
-                                                                forall `{GHC.Prim.Ord a}, Data.Monoid.Dual a -> a :=
-  fun {a} `{GHC.Prim.Ord a} => getDual.
+                                                                forall `{GHC.Base.Ord a}, Data.Monoid.Dual a -> a :=
+  fun {a} `{GHC.Base.Ord a} => getDual.
 
 Local Definition instance_Foldable_Data_Monoid_Dual_minimum : forall {a},
-                                                                forall `{GHC.Prim.Ord a}, Data.Monoid.Dual a -> a :=
-  fun {a} `{GHC.Prim.Ord a} => getDual.
+                                                                forall `{GHC.Base.Ord a}, Data.Monoid.Dual a -> a :=
+  fun {a} `{GHC.Base.Ord a} => getDual.
 
 Local Definition instance_Foldable_Data_Monoid_Dual_null : forall {a},
                                                              Data.Monoid.Dual a -> bool :=
@@ -603,28 +601,28 @@ Local Definition instance_Foldable_Data_Monoid_Dual_toList : forall {a},
     fun arg_249__ => match arg_249__ with | (Data.Monoid.Dual x) => cons x nil end.
 
 Local Definition instance_Foldable_Data_Monoid_Sum_elem : forall {a},
-                                                            forall `{GHC.Prim.Eq_ a}, a -> Data.Monoid.Sum a -> bool :=
-  fun {a} `{GHC.Prim.Eq_ a} =>
+                                                            forall `{GHC.Base.Eq_ a}, a -> Data.Monoid.Sum a -> bool :=
+  fun {a} `{GHC.Base.Eq_ a} =>
     hashDot (fun arg_220__ => Coq.Program.Basics.compose arg_220__ getSum)
-            GHC.Prim.op_zeze__.
+            GHC.Base.op_zeze__.
 
 Local Definition instance_Foldable_Data_Monoid_Sum_foldMap : forall {m} {a},
-                                                               forall `{GHC.BaseGen.Monoid m},
+                                                               forall `{GHC.Base.Monoid m},
                                                                  (a -> m) -> Data.Monoid.Sum a -> m :=
-  fun {m} {a} `{GHC.BaseGen.Monoid m} => GHC.Prim.coerce.
+  fun {m} {a} `{GHC.Base.Monoid m} => GHC.Base.coerce.
 
 Local Definition instance_Foldable_Data_Monoid_Sum_fold : forall {m},
-                                                            forall `{GHC.BaseGen.Monoid m}, Data.Monoid.Sum m -> m :=
-  fun {m} `{GHC.BaseGen.Monoid m} =>
-    instance_Foldable_Data_Monoid_Sum_foldMap GHC.BaseGen.id.
+                                                            forall `{GHC.Base.Monoid m}, Data.Monoid.Sum m -> m :=
+  fun {m} `{GHC.Base.Monoid m} =>
+    instance_Foldable_Data_Monoid_Sum_foldMap GHC.Base.id.
 
 Local Definition instance_Foldable_Data_Monoid_Sum_foldl : forall {b} {a},
                                                              (b -> a -> b) -> b -> Data.Monoid.Sum a -> b :=
-  fun {b} {a} => GHC.Prim.coerce.
+  fun {b} {a} => GHC.Base.coerce.
 
 Local Definition instance_Foldable_Data_Monoid_Sum_foldl' : forall {b} {a},
                                                               (b -> a -> b) -> b -> Data.Monoid.Sum a -> b :=
-  fun {b} {a} => GHC.Prim.coerce.
+  fun {b} {a} => GHC.Base.coerce.
 
 Local Definition instance_Foldable_Data_Monoid_Sum_foldl1 : forall {a},
                                                               (a -> a -> a) -> Data.Monoid.Sum a -> a :=
@@ -651,12 +649,12 @@ Local Definition instance_Foldable_Data_Monoid_Sum_length : forall {a},
   fun {a} => fun arg_229__ => one.
 
 Local Definition instance_Foldable_Data_Monoid_Sum_maximum : forall {a},
-                                                               forall `{GHC.Prim.Ord a}, Data.Monoid.Sum a -> a :=
-  fun {a} `{GHC.Prim.Ord a} => getSum.
+                                                               forall `{GHC.Base.Ord a}, Data.Monoid.Sum a -> a :=
+  fun {a} `{GHC.Base.Ord a} => getSum.
 
 Local Definition instance_Foldable_Data_Monoid_Sum_minimum : forall {a},
-                                                               forall `{GHC.Prim.Ord a}, Data.Monoid.Sum a -> a :=
-  fun {a} `{GHC.Prim.Ord a} => getSum.
+                                                               forall `{GHC.Base.Ord a}, Data.Monoid.Sum a -> a :=
+  fun {a} `{GHC.Base.Ord a} => getSum.
 
 Local Definition instance_Foldable_Data_Monoid_Sum_null : forall {a},
                                                             Data.Monoid.Sum a -> bool :=
@@ -676,30 +674,30 @@ Local Definition instance_Foldable_Data_Monoid_Sum_toList : forall {a},
     fun arg_233__ => match arg_233__ with | (Data.Monoid.Sum x) => cons x nil end.
 
 Local Definition instance_Foldable_Data_Monoid_Product_elem : forall {a},
-                                                                forall `{GHC.Prim.Eq_ a},
+                                                                forall `{GHC.Base.Eq_ a},
                                                                   a -> Data.Monoid.Product a -> bool :=
-  fun {a} `{GHC.Prim.Eq_ a} =>
+  fun {a} `{GHC.Base.Eq_ a} =>
     hashDot (fun arg_204__ => Coq.Program.Basics.compose arg_204__ getProduct)
-            GHC.Prim.op_zeze__.
+            GHC.Base.op_zeze__.
 
 Local Definition instance_Foldable_Data_Monoid_Product_foldMap : forall {m} {a},
-                                                                   forall `{GHC.BaseGen.Monoid m},
+                                                                   forall `{GHC.Base.Monoid m},
                                                                      (a -> m) -> Data.Monoid.Product a -> m :=
-  fun {m} {a} `{GHC.BaseGen.Monoid m} => GHC.Prim.coerce.
+  fun {m} {a} `{GHC.Base.Monoid m} => GHC.Base.coerce.
 
 Local Definition instance_Foldable_Data_Monoid_Product_fold : forall {m},
-                                                                forall `{GHC.BaseGen.Monoid m},
+                                                                forall `{GHC.Base.Monoid m},
                                                                   Data.Monoid.Product m -> m :=
-  fun {m} `{GHC.BaseGen.Monoid m} =>
-    instance_Foldable_Data_Monoid_Product_foldMap GHC.BaseGen.id.
+  fun {m} `{GHC.Base.Monoid m} =>
+    instance_Foldable_Data_Monoid_Product_foldMap GHC.Base.id.
 
 Local Definition instance_Foldable_Data_Monoid_Product_foldl : forall {b} {a},
                                                                  (b -> a -> b) -> b -> Data.Monoid.Product a -> b :=
-  fun {b} {a} => GHC.Prim.coerce.
+  fun {b} {a} => GHC.Base.coerce.
 
 Local Definition instance_Foldable_Data_Monoid_Product_foldl' : forall {b} {a},
                                                                   (b -> a -> b) -> b -> Data.Monoid.Product a -> b :=
-  fun {b} {a} => GHC.Prim.coerce.
+  fun {b} {a} => GHC.Base.coerce.
 
 Local Definition instance_Foldable_Data_Monoid_Product_foldl1 : forall {a},
                                                                   (a -> a -> a) -> Data.Monoid.Product a -> a :=
@@ -726,14 +724,14 @@ Local Definition instance_Foldable_Data_Monoid_Product_length : forall {a},
   fun {a} => fun arg_213__ => one.
 
 Local Definition instance_Foldable_Data_Monoid_Product_maximum : forall {a},
-                                                                   forall `{GHC.Prim.Ord a},
+                                                                   forall `{GHC.Base.Ord a},
                                                                      Data.Monoid.Product a -> a :=
-  fun {a} `{GHC.Prim.Ord a} => getProduct.
+  fun {a} `{GHC.Base.Ord a} => getProduct.
 
 Local Definition instance_Foldable_Data_Monoid_Product_minimum : forall {a},
-                                                                   forall `{GHC.Prim.Ord a},
+                                                                   forall `{GHC.Base.Ord a},
                                                                      Data.Monoid.Product a -> a :=
-  fun {a} `{GHC.Prim.Ord a} => getProduct.
+  fun {a} `{GHC.Base.Ord a} => getProduct.
 
 Local Definition instance_Foldable_Data_Monoid_Product_null : forall {a},
                                                                 Data.Monoid.Product a -> bool :=
@@ -759,9 +757,9 @@ Local Definition instance_Foldable_Data_Monoid_Product_toList : forall {a},
 
 (*
 Local Definition instance_Foldable_Data_Monoid_First_foldMap : forall {m} {a},
-                                                                 forall `{GHC.BaseGen.Monoid m},
+                                                                 forall `{GHC.Base.Monoid m},
                                                                    (a -> m) -> Data.Monoid.First a -> m :=
-  fun {m} {a} `{GHC.BaseGen.Monoid m} =>
+  fun {m} {a} `{GHC.Base.Monoid m} =>
     fix foldMap arg_201__
           := match arg_201__ with
                | f => Coq.Program.Basics.compose (foldMap f) Data.Monoid.getFirst
@@ -774,7 +772,7 @@ Local Definition instance_Foldable_Data_Monoid_First_foldl : forall {b} {a},
       match arg_19__ , arg_20__ , arg_21__ with
         | f , z , t => appEndo (getDual (instance_Foldable_Data_Monoid_First_foldMap
                                         (Coq.Program.Basics.compose Data.Monoid.Dual (Coq.Program.Basics.compose
-                                                                    Data.Monoid.Endo (GHC.BaseGen.flip f))) t)) z
+                                                                    Data.Monoid.Endo (GHC.Base.flip f))) t)) z
       end.
 
 Local Definition instance_Foldable_Data_Monoid_First_foldl1 : forall {a},
@@ -787,7 +785,7 @@ Local Definition instance_Foldable_Data_Monoid_First_foldl1 : forall {a},
                         match arg_46__ , arg_47__ with
                           | m , y => Some (match m with | None => y | (Some x) => f x y end)
                         end in
-                    Data.Maybe.fromMaybe (GHC.Prim.errorWithoutStackTrace
+                    Data.Maybe.fromMaybe (GHC.Base.errorWithoutStackTrace
                                          &"foldl1: empty structure") (instance_Foldable_Data_Monoid_First_foldl mf None
                                                                      xs)
       end.
@@ -802,7 +800,7 @@ Local Definition instance_Foldable_Data_Monoid_First_foldr' : forall {a} {b},
                              match arg_12__ , arg_13__ , arg_14__ with
                                | k , x , z => GHC.Base.op_zdzn__ k (f x z)
                              end in
-                         instance_Foldable_Data_Monoid_First_foldl f' GHC.BaseGen.id xs z0
+                         instance_Foldable_Data_Monoid_First_foldl f' GHC.Base.id xs z0
       end.
 
 Local Definition instance_Foldable_Data_Monoid_First_foldr : forall {a} {b},
@@ -824,7 +822,7 @@ Local Definition instance_Foldable_Data_Monoid_First_foldl' : forall {b} {a},
                              match arg_27__ , arg_28__ , arg_29__ with
                                | x , k , z => GHC.Base.op_zdzn__ k (f z x)
                              end in
-                         instance_Foldable_Data_Monoid_First_foldr f' GHC.BaseGen.id xs z0
+                         instance_Foldable_Data_Monoid_First_foldr f' GHC.Base.id xs z0
       end.
 
 Local Definition instance_Foldable_Data_Monoid_First_length : forall {a},
@@ -845,7 +843,7 @@ Local Definition instance_Foldable_Data_Monoid_First_foldr1 : forall {a},
                         match arg_36__ , arg_37__ with
                           | x , m => Some (match m with | None => x | (Some y) => f x y end)
                         end in
-                    Data.Maybe.fromMaybe (GHC.Prim.errorWithoutStackTrace
+                    Data.Maybe.fromMaybe (GHC.Base.errorWithoutStackTrace
                                          &"foldr1: empty structure") (instance_Foldable_Data_Monoid_First_foldr mf None
                                                                      xs)
       end.
@@ -860,7 +858,7 @@ Local Definition instance_Foldable_Data_Monoid_First_toList : forall {a},
   fun {a} =>
     fun arg_54__ =>
       match arg_54__ with
-        | t => Prim.build (fun arg_55__ arg_56__ =>
+        | t => Base.build (fun arg_55__ arg_56__ =>
                                 match arg_55__ , arg_56__ with
                                   | c , n => instance_Foldable_Data_Monoid_First_foldr c n t
                                 end)
@@ -878,15 +876,15 @@ Local Definition instance_Foldable_Data_Monoid_First_sum : forall {a},
     hashDot getSum (instance_Foldable_Data_Monoid_First_foldMap Data.Monoid.Sum).
 
 Local Definition instance_Foldable_Data_Monoid_First_fold : forall {m},
-                                                              forall `{GHC.BaseGen.Monoid m},
+                                                              forall `{GHC.Base.Monoid m},
                                                                 Data.Monoid.First m -> m :=
-  fun {m} `{GHC.BaseGen.Monoid m} =>
-    instance_Foldable_Data_Monoid_First_foldMap GHC.BaseGen.id.
+  fun {m} `{GHC.Base.Monoid m} =>
+    instance_Foldable_Data_Monoid_First_foldMap GHC.Base.id.
 
 Local Definition instance_Foldable_Data_Monoid_Last_foldMap : forall {m} {a},
-                                                                forall `{GHC.BaseGen.Monoid m},
+                                                                forall `{GHC.Base.Monoid m},
                                                                   (a -> m) -> Data.Monoid.Last a -> m :=
-  fun {m} {a} `{GHC.BaseGen.Monoid m} =>
+  fun {m} {a} `{GHC.Base.Monoid m} =>
     fix foldMap arg_198__
           := match arg_198__ with
                | f => Coq.Program.Basics.compose (foldMap f) getLast
@@ -899,7 +897,7 @@ Local Definition instance_Foldable_Data_Monoid_Last_foldl : forall {b} {a},
       match arg_19__ , arg_20__ , arg_21__ with
         | f , z , t => appEndo (getDual (instance_Foldable_Data_Monoid_Last_foldMap
                                         (Coq.Program.Basics.compose Data.Monoid.Dual (Coq.Program.Basics.compose
-                                                                    Data.Monoid.Endo (GHC.BaseGen.flip f))) t)) z
+                                                                    Data.Monoid.Endo (GHC.Base.flip f))) t)) z
       end.
 
 Local Definition instance_Foldable_Data_Monoid_Last_foldl1 : forall {a},
@@ -912,7 +910,7 @@ Local Definition instance_Foldable_Data_Monoid_Last_foldl1 : forall {a},
                         match arg_46__ , arg_47__ with
                           | m , y => Some (match m with | None => y | (Some x) => f x y end)
                         end in
-                    Data.Maybe.fromMaybe (GHC.Prim.errorWithoutStackTrace
+                    Data.Maybe.fromMaybe (GHC.Base.errorWithoutStackTrace
                                          &"foldl1: empty structure") (instance_Foldable_Data_Monoid_Last_foldl mf None
                                                                      xs)
       end.
@@ -927,7 +925,7 @@ Local Definition instance_Foldable_Data_Monoid_Last_foldr' : forall {a} {b},
                              match arg_12__ , arg_13__ , arg_14__ with
                                | k , x , z => GHC.Base.op_zdzn__ k (f x z)
                              end in
-                         instance_Foldable_Data_Monoid_Last_foldl f' GHC.BaseGen.id xs z0
+                         instance_Foldable_Data_Monoid_Last_foldl f' GHC.Base.id xs z0
       end.
 
 Local Definition instance_Foldable_Data_Monoid_Last_foldr : forall {a} {b},
@@ -949,7 +947,7 @@ Local Definition instance_Foldable_Data_Monoid_Last_foldl' : forall {b} {a},
                              match arg_27__ , arg_28__ , arg_29__ with
                                | x , k , z => GHC.Base.op_zdzn__ k (f z x)
                              end in
-                         instance_Foldable_Data_Monoid_Last_foldr f' GHC.BaseGen.id xs z0
+                         instance_Foldable_Data_Monoid_Last_foldr f' GHC.Base.id xs z0
       end.
 
 Local Definition instance_Foldable_Data_Monoid_Last_length : forall {a},
@@ -970,7 +968,7 @@ Local Definition instance_Foldable_Data_Monoid_Last_foldr1 : forall {a},
                         match arg_36__ , arg_37__ with
                           | x , m => Some (match m with | None => x | (Some y) => f x y end)
                         end in
-                    Data.Maybe.fromMaybe (GHC.Prim.errorWithoutStackTrace
+                    Data.Maybe.fromMaybe (GHC.Base.errorWithoutStackTrace
                                          &"foldr1: empty structure") (instance_Foldable_Data_Monoid_Last_foldr mf None
                                                                      xs)
       end.
@@ -985,7 +983,7 @@ Local Definition instance_Foldable_Data_Monoid_Last_toList : forall {a},
   fun {a} =>
     fun arg_54__ =>
       match arg_54__ with
-        | t => Prim.build (fun arg_55__ arg_56__ =>
+        | t => Base.build (fun arg_55__ arg_56__ =>
                                 match arg_55__ , arg_56__ with
                                   | c , n => instance_Foldable_Data_Monoid_Last_foldr c n t
                                 end)
@@ -1003,29 +1001,29 @@ Local Definition instance_Foldable_Data_Monoid_Last_sum : forall {a},
     hashDot getSum (instance_Foldable_Data_Monoid_Last_foldMap Data.Monoid.Sum).
 
 Local Definition instance_Foldable_Data_Monoid_Last_fold : forall {m},
-                                                             forall `{GHC.BaseGen.Monoid m}, Data.Monoid.Last m -> m :=
-  fun {m} `{GHC.BaseGen.Monoid m} =>
-    instance_Foldable_Data_Monoid_Last_foldMap GHC.BaseGen.id.
+                                                             forall `{GHC.Base.Monoid m}, Data.Monoid.Last m -> m :=
+  fun {m} `{GHC.Base.Monoid m} =>
+    instance_Foldable_Data_Monoid_Last_foldMap GHC.Base.id.
 *)
-(* Translating `instance forall `{GHC.Prim.Ord a}, GHC.BaseGen.Monoid (Max a)'
+(* Translating `instance forall `{GHC.Base.Ord a}, GHC.Base.Monoid (Max a)'
    failed: OOPS! Cannot construct types for this class def: Nothing unsupported *)
 
-(* Translating `instance forall `{GHC.Prim.Ord a}, GHC.BaseGen.Monoid (Min a)'
+(* Translating `instance forall `{GHC.Base.Ord a}, GHC.Base.Monoid (Min a)'
    failed: OOPS! Cannot construct types for this class def: Nothing unsupported *)
 
 (*
 Local Definition instance_Foldable_GHC_Generics_U1_elem : forall {a},
-                                                            forall `{GHC.Prim.Eq_ a}, a -> GHC.Generics.U1 a -> bool :=
-  fun {a} `{GHC.Prim.Eq_ a} => fun arg_190__ arg_191__ => false.
+                                                            forall `{GHC.Base.Eq_ a}, a -> GHC.Generics.U1 a -> bool :=
+  fun {a} `{GHC.Base.Eq_ a} => fun arg_190__ arg_191__ => false.
 
 Local Definition instance_Foldable_GHC_Generics_U1_fold : forall {m},
-                                                            forall `{GHC.BaseGen.Monoid m}, GHC.Generics.U1 m -> m :=
-  fun {m} `{GHC.BaseGen.Monoid m} => fun arg_169__ => GHC.Base.mempty.
+                                                            forall `{GHC.Base.Monoid m}, GHC.Generics.U1 m -> m :=
+  fun {m} `{GHC.Base.Monoid m} => fun arg_169__ => GHC.Base.mempty.
 
 Local Definition instance_Foldable_GHC_Generics_U1_foldMap : forall {m} {a},
-                                                               forall `{GHC.BaseGen.Monoid m},
+                                                               forall `{GHC.Base.Monoid m},
                                                                  (a -> m) -> GHC.Generics.U1 a -> m :=
-  fun {m} {a} `{GHC.BaseGen.Monoid m} =>
+  fun {m} {a} `{GHC.Base.Monoid m} =>
     fun arg_167__ arg_168__ => GHC.Base.mempty.
 
 Local Definition instance_Foldable_GHC_Generics_U1_foldl : forall {b} {a},
@@ -1046,13 +1044,13 @@ Local Definition instance_Foldable_GHC_Generics_U1_foldr' : forall {a} {b},
                              match arg_12__ , arg_13__ , arg_14__ with
                                | k , x , z => GHC.Base.op_zdzn__ k (f x z)
                              end in
-                         instance_Foldable_GHC_Generics_U1_foldl f' GHC.BaseGen.id xs z0
+                         instance_Foldable_GHC_Generics_U1_foldl f' GHC.Base.id xs z0
       end.
 
 Local Definition instance_Foldable_GHC_Generics_U1_foldl1 : forall {a},
                                                               (a -> a -> a) -> GHC.Generics.U1 a -> a :=
   fun {a} =>
-    fun arg_178__ arg_179__ => GHC.Prim.errorWithoutStackTrace &"foldl1: U1".
+    fun arg_178__ arg_179__ => GHC.Base.errorWithoutStackTrace &"foldl1: U1".
 
 Local Definition instance_Foldable_GHC_Generics_U1_foldr : forall {a} {b},
                                                              (a -> b -> b) -> b -> GHC.Generics.U1 a -> b :=
@@ -1067,7 +1065,7 @@ Local Definition instance_Foldable_GHC_Generics_U1_toList : forall {a},
   fun {a} =>
     fun arg_54__ =>
       match arg_54__ with
-        | t => Prim.build (fun arg_55__ arg_56__ =>
+        | t => Base.build (fun arg_55__ arg_56__ =>
                                 match arg_55__ , arg_56__ with
                                   | c , n => instance_Foldable_GHC_Generics_U1_foldr c n t
                                 end)
@@ -1083,13 +1081,13 @@ Local Definition instance_Foldable_GHC_Generics_U1_foldl' : forall {b} {a},
                              match arg_27__ , arg_28__ , arg_29__ with
                                | x , k , z => GHC.Base.op_zdzn__ k (f z x)
                              end in
-                         instance_Foldable_GHC_Generics_U1_foldr f' GHC.BaseGen.id xs z0
+                         instance_Foldable_GHC_Generics_U1_foldr f' GHC.Base.id xs z0
       end.
 
 Local Definition instance_Foldable_GHC_Generics_U1_foldr1 : forall {a},
                                                               (a -> a -> a) -> GHC.Generics.U1 a -> a :=
   fun {a} =>
-    fun arg_182__ arg_183__ => GHC.Prim.errorWithoutStackTrace &"foldr1: U1".
+    fun arg_182__ arg_183__ => GHC.Base.errorWithoutStackTrace &"foldr1: U1".
 
 Local Definition instance_Foldable_GHC_Generics_U1_length : forall {a},
                                                               GHC.Generics.U1 a -> GHC.Num.Int :=
@@ -1110,15 +1108,15 @@ Local Definition instance_Foldable_GHC_Generics_U1_sum : forall {a},
 *)
 (*
 Local Definition instance_Foldable__GHC_Tuple_____a__fold {a} : forall {m},
-                                                              forall `{GHC.BaseGen.Monoid m},
+                                                              forall `{GHC.Base.Monoid m},
                                                                 (a * m) -> m :=
-  fun {m} `{GHC.BaseGen.Monoid m} =>
-    instance_Foldable__GHC_Tuple_____a__foldMap GHC.BaseGen.id.
+  fun {m} `{GHC.Base.Monoid m} =>
+    instance_Foldable__GHC_Tuple_____a__foldMap GHC.Base.id.
 *)
 Class Foldable t := {
-  elem : forall {a}, forall `{GHC.Prim.Eq_ a}, a -> t a -> bool ;
-  fold : forall {m}, forall `{GHC.BaseGen.Monoid m}, t m -> m ;
-  foldMap : forall {m} {a}, forall `{GHC.BaseGen.Monoid m}, (a -> m) -> t a -> m ;
+  elem : forall {a}, forall `{GHC.Base.Eq_ a}, a -> t a -> bool ;
+  fold : forall {m}, forall `{GHC.Base.Monoid m}, t m -> m ;
+  foldMap : forall {m} {a}, forall `{GHC.Base.Monoid m}, (a -> m) -> t a -> m ;
   foldl : forall {b} {a}, (b -> a -> b) -> b -> t a -> b ;
   foldl' : forall {b} {a}, (b -> a -> b) -> b -> t a -> b ;
   foldl1 : forall {a}, (a -> a -> a) -> t a -> a ;
@@ -1126,34 +1124,34 @@ Class Foldable t := {
   foldr' : forall {a} {b}, (a -> b -> b) -> b -> t a -> b ;
   foldr1 : forall {a}, (a -> a -> a) -> t a -> a ;
   length : forall {a}, t a -> GHC.Num.Int ;
-  maximum : forall {a}, forall `{GHC.Prim.Ord a}, t a -> a ;
-  minimum : forall {a}, forall `{GHC.Prim.Ord a}, t a -> a ;
+  maximum : forall {a}, forall `{GHC.Base.Ord a}, t a -> a ;
+  minimum : forall {a}, forall `{GHC.Base.Ord a}, t a -> a ;
   null : forall {a}, t a -> bool ;
   product : forall {a}, forall `{GHC.Num.Num a}, t a -> a ;
   sum : forall {a}, forall `{GHC.Num.Num a}, t a -> a ;
   toList : forall {a}, t a -> list a }.
 
-Definition traverse_ {t} {f} {a} {b} `{Foldable t} `{GHC.BaseGen.Applicative f}
+Definition traverse_ {t} {f} {a} {b} `{Foldable t} `{GHC.Base.Applicative f}
     : (a -> f b) -> t a -> f unit :=
   fun arg_143__ =>
     match arg_143__ with
-      | f => foldr (Coq.Program.Basics.compose GHC.BaseGen.op_ztzg__ f) (GHC.BaseGen.pure
+      | f => foldr (Coq.Program.Basics.compose GHC.Base.op_ztzg__ f) (GHC.Base.pure
                                                                      tt)
     end.
 
-Definition sequence_ {t} {m} {a} `{Foldable t} `{GHC.BaseGen.Monad m} : t (m
+Definition sequence_ {t} {m} {a} `{Foldable t} `{GHC.Base.Monad m} : t (m
                                                                           a) -> m unit :=
-  foldr GHC.BaseGen.op_zgzg__ (GHC.BaseGen.return_ tt).
+  foldr GHC.Base.op_zgzg__ (GHC.Base.return_ tt).
 
-Definition sequenceA_ {t} {f} {a} `{Foldable t} `{GHC.BaseGen.Applicative f} : t
+Definition sequenceA_ {t} {f} {a} `{Foldable t} `{GHC.Base.Applicative f} : t
                                                                                (f a) -> f unit :=
-  foldr GHC.BaseGen.op_ztzg__ (GHC.BaseGen.pure tt).
+  foldr GHC.Base.op_ztzg__ (GHC.Base.pure tt).
 
 (*
 Definition or {t} `{Foldable t} : t bool -> bool :=
   hashDot getAny (foldMap Data.Monoid.Any).
 *)
-Definition notElem {t} {a} `{Foldable t} `{GHC.Prim.Eq_ a} : a -> t a -> bool :=
+Definition notElem {t} {a} `{Foldable t} `{GHC.Base.Eq_ a} : a -> t a -> bool :=
   fun arg_84__ =>
     match arg_84__ with
       | x => Coq.Program.Basics.compose negb (elem x)
@@ -1191,44 +1189,44 @@ Definition maximumBy {t} {a} `{Foldable t} : (a -> a -> comparison) -> t
                foldr1 max'
     end.
 
-Definition mapM_ {t} {m} {a} {b} `{Foldable t} `{GHC.BaseGen.Monad m} : (a -> m
+Definition mapM_ {t} {m} {a} {b} `{Foldable t} `{GHC.Base.Monad m} : (a -> m
                                                                         b) -> t a -> m unit :=
   fun arg_139__ =>
     match arg_139__ with
-      | f => foldr (Coq.Program.Basics.compose GHC.BaseGen.op_zgzg__ f) (GHC.BaseGen.return_
+      | f => foldr (Coq.Program.Basics.compose GHC.Base.op_zgzg__ f) (GHC.Base.return_
                                                                      tt)
     end.
 
-Definition for_ {t} {f} {a} {b} `{Foldable t} `{GHC.BaseGen.Applicative f} : t
+Definition for_ {t} {f} {a} {b} `{Foldable t} `{GHC.Base.Applicative f} : t
                                                                              a -> (a -> f b) -> f unit :=
-  GHC.BaseGen.flip traverse_.
+  GHC.Base.flip traverse_.
 
-Definition forM_ {t} {m} {a} {b} `{Foldable t} `{GHC.BaseGen.Monad m} : t
+Definition forM_ {t} {m} {a} {b} `{Foldable t} `{GHC.Base.Monad m} : t
                                                                         a -> (a -> m b) -> m unit :=
-  GHC.BaseGen.flip mapM_.
+  GHC.Base.flip mapM_.
 
-Definition foldrM {t} {m} {a} {b} `{Foldable t} `{GHC.BaseGen.Monad m}
+Definition foldrM {t} {m} {a} {b} `{Foldable t} `{GHC.Base.Monad m}
     : (a -> b -> m b) -> b -> t a -> m b :=
   fun arg_157__ arg_158__ arg_159__ =>
     match arg_157__ , arg_158__ , arg_159__ with
       | f , z0 , xs => let f' :=
                          fun arg_160__ arg_161__ arg_162__ =>
                            match arg_160__ , arg_161__ , arg_162__ with
-                             | k , x , z => GHC.BaseGen.op_zgzgze__ (f x z) k
+                             | k , x , z => GHC.Base.op_zgzgze__ (f x z) k
                            end in
-                       foldl f' GHC.BaseGen.return_ xs z0
+                       foldl f' GHC.Base.return_ xs z0
     end.
 
-Definition foldlM {t} {m} {b} {a} `{Foldable t} `{GHC.BaseGen.Monad m}
+Definition foldlM {t} {m} {b} {a} `{Foldable t} `{GHC.Base.Monad m}
     : (b -> a -> m b) -> b -> t a -> m b :=
   fun arg_147__ arg_148__ arg_149__ =>
     match arg_147__ , arg_148__ , arg_149__ with
       | f , z0 , xs => let f' :=
                          fun arg_150__ arg_151__ arg_152__ =>
                            match arg_150__ , arg_151__ , arg_152__ with
-                             | x , k , z => GHC.BaseGen.op_zgzgze__ (f z x) k
+                             | x , k , z => GHC.Base.op_zgzgze__ (f z x) k
                            end in
-                       foldr f' GHC.BaseGen.return_ xs z0
+                       foldr f' GHC.Base.return_ xs z0
     end.
 
 Definition find {t} {a} `{Foldable t} : (a -> bool) -> t a -> option a :=
@@ -1242,11 +1240,11 @@ Definition find {t} {a} `{Foldable t} : (a -> bool) -> t a -> option a :=
     end.
 
 
-Definition asum {t} {f} {a} `{Foldable t} `{GHC.BaseGen.Alternative f} : t (f
+Definition asum {t} {f} {a} `{Foldable t} `{GHC.Base.Alternative f} : t (f
                                                                            a) -> f a :=
-  foldr GHC.BaseGen.op_zlzbzg__ GHC.BaseGen.empty.
+  foldr GHC.Base.op_zlzbzg__ GHC.Base.empty.
 
-Definition msum {t} {m} {a} `{Foldable t} `{GHC.BaseGen.MonadPlus m} : t (m a) -> m
+Definition msum {t} {m} {a} `{Foldable t} `{GHC.Base.MonadPlus m} : t (m a) -> m
                                                                     a :=
   asum.
 
@@ -1258,29 +1256,29 @@ Definition any {t} {a} `{Foldable t} : (a -> bool) -> t a -> bool :=
     end.
 (*
 Local Definition instance_Foldable_Data_Monoid_Last_elem : forall {a},
-                                                             forall `{GHC.Prim.Eq_ a},
+                                                             forall `{GHC.Base.Eq_ a},
                                                                a -> Data.Monoid.Last a -> bool :=
-  fun {a} `{GHC.Prim.Eq_ a} => Coq.Program.Basics.compose any GHC.Prim.op_zeze__.
+  fun {a} `{GHC.Base.Eq_ a} => Coq.Program.Basics.compose any GHC.Base.op_zeze__.
 
 Local Definition instance_Foldable_Data_Monoid_First_elem : forall {a},
-                                                              forall `{GHC.Prim.Eq_ a},
+                                                              forall `{GHC.Base.Eq_ a},
                                                                 a -> Data.Monoid.First a -> bool :=
-  fun {a} `{GHC.Prim.Eq_ a} => Coq.Program.Basics.compose any GHC.Prim.op_zeze__.
+  fun {a} `{GHC.Base.Eq_ a} => Coq.Program.Basics.compose any GHC.Base.op_zeze__.
 
 Local Definition instance_Foldable__GHC_Arr_Array_i__elem : forall {a},
-                                                              forall `{GHC.Prim.Eq_ a},
+                                                              forall `{GHC.Base.Eq_ a},
                                                                 a -> (GHC.Arr.Array i) a -> bool :=
-  fun {a} `{GHC.Prim.Eq_ a} => Coq.Program.Basics.compose any GHC.Prim.op_zeze__.
+  fun {a} `{GHC.Base.Eq_ a} => Coq.Program.Basics.compose any GHC.Base.op_zeze__.
 
 Local Definition instance_Foldable__GHC_Tuple_____a__elem : forall {a},
-                                                              forall `{GHC.Prim.Eq_ a},
+                                                              forall `{GHC.Base.Eq_ a},
                                                                 a -> (GHC.Tuple.[,] a) a -> bool :=
-  fun {a} `{GHC.Prim.Eq_ a} => Coq.Program.Basics.compose any GHC.Prim.op_zeze__.
+  fun {a} `{GHC.Base.Eq_ a} => Coq.Program.Basics.compose any GHC.Base.op_zeze__.
 *)
 
 (*Local Definition instance_Foldable_option_elem : forall {a},
-                                                   forall `{GHC.Prim.Eq_ a}, a -> option a -> bool :=
-  fun {a} `{GHC.Prim.Eq_ a} => Coq.Program.Basics.compose any GHC.Prim.op_zeze__. *)
+                                                   forall `{GHC.Base.Eq_ a}, a -> option a -> bool :=
+  fun {a} `{GHC.Base.Eq_ a} => Coq.Program.Basics.compose any GHC.Base.op_zeze__. *)
 (*
 Definition and {t} `{Foldable t} : t bool -> bool :=
   hashDot getAll (foldMap Data.Monoid.All).
@@ -1294,11 +1292,11 @@ Definition all {t} {a} `{Foldable t} : (a -> bool) -> t a -> bool :=
 (*
 Instance instance_Foldable_Data_Monoid_Product : !Foldable
                                                  Data.Monoid.Product := {
-  elem := fun {a} `{GHC.Prim.Eq_ a} =>
+  elem := fun {a} `{GHC.Base.Eq_ a} =>
     instance_Foldable_Data_Monoid_Product_elem ;
-  fold := fun {m} `{GHC.BaseGen.Monoid m} =>
+  fold := fun {m} `{GHC.Base.Monoid m} =>
     instance_Foldable_Data_Monoid_Product_fold ;
-  foldMap := fun {m} {a} `{GHC.BaseGen.Monoid m} =>
+  foldMap := fun {m} {a} `{GHC.Base.Monoid m} =>
     instance_Foldable_Data_Monoid_Product_foldMap ;
   foldl := fun {b} {a} => instance_Foldable_Data_Monoid_Product_foldl ;
   foldl' := fun {b} {a} => instance_Foldable_Data_Monoid_Product_foldl' ;
@@ -1307,9 +1305,9 @@ Instance instance_Foldable_Data_Monoid_Product : !Foldable
   foldr' := fun {a} {b} => instance_Foldable_Data_Monoid_Product_foldr' ;
   foldr1 := fun {a} => instance_Foldable_Data_Monoid_Product_foldr1 ;
   length := fun {a} => instance_Foldable_Data_Monoid_Product_length ;
-  maximum := fun {a} `{GHC.Prim.Ord a} =>
+  maximum := fun {a} `{GHC.Base.Ord a} =>
     instance_Foldable_Data_Monoid_Product_maximum ;
-  minimum := fun {a} `{GHC.Prim.Ord a} =>
+  minimum := fun {a} `{GHC.Base.Ord a} =>
     instance_Foldable_Data_Monoid_Product_minimum ;
   null := fun {a} => instance_Foldable_Data_Monoid_Product_null ;
   product := fun {a} `{GHC.Num.Num a} =>
@@ -1318,10 +1316,10 @@ Instance instance_Foldable_Data_Monoid_Product : !Foldable
   toList := fun {a} => instance_Foldable_Data_Monoid_Product_toList }.
 
 Instance instance_Foldable_Data_Monoid_Sum : !Foldable Data.Monoid.Sum := {
-  elem := fun {a} `{GHC.Prim.Eq_ a} => instance_Foldable_Data_Monoid_Sum_elem ;
-  fold := fun {m} `{GHC.BaseGen.Monoid m} =>
+  elem := fun {a} `{GHC.Base.Eq_ a} => instance_Foldable_Data_Monoid_Sum_elem ;
+  fold := fun {m} `{GHC.Base.Monoid m} =>
     instance_Foldable_Data_Monoid_Sum_fold ;
-  foldMap := fun {m} {a} `{GHC.BaseGen.Monoid m} =>
+  foldMap := fun {m} {a} `{GHC.Base.Monoid m} =>
     instance_Foldable_Data_Monoid_Sum_foldMap ;
   foldl := fun {b} {a} => instance_Foldable_Data_Monoid_Sum_foldl ;
   foldl' := fun {b} {a} => instance_Foldable_Data_Monoid_Sum_foldl' ;
@@ -1330,9 +1328,9 @@ Instance instance_Foldable_Data_Monoid_Sum : !Foldable Data.Monoid.Sum := {
   foldr' := fun {a} {b} => instance_Foldable_Data_Monoid_Sum_foldr' ;
   foldr1 := fun {a} => instance_Foldable_Data_Monoid_Sum_foldr1 ;
   length := fun {a} => instance_Foldable_Data_Monoid_Sum_length ;
-  maximum := fun {a} `{GHC.Prim.Ord a} =>
+  maximum := fun {a} `{GHC.Base.Ord a} =>
     instance_Foldable_Data_Monoid_Sum_maximum ;
-  minimum := fun {a} `{GHC.Prim.Ord a} =>
+  minimum := fun {a} `{GHC.Base.Ord a} =>
     instance_Foldable_Data_Monoid_Sum_minimum ;
   null := fun {a} => instance_Foldable_Data_Monoid_Sum_null ;
   product := fun {a} `{GHC.Num.Num a} =>
@@ -1341,10 +1339,10 @@ Instance instance_Foldable_Data_Monoid_Sum : !Foldable Data.Monoid.Sum := {
   toList := fun {a} => instance_Foldable_Data_Monoid_Sum_toList }.
 
 Instance instance_Foldable_Data_Monoid_Dual : !Foldable Data.Monoid.Dual := {
-  elem := fun {a} `{GHC.Prim.Eq_ a} => instance_Foldable_Data_Monoid_Dual_elem ;
-  fold := fun {m} `{GHC.BaseGen.Monoid m} =>
+  elem := fun {a} `{GHC.Base.Eq_ a} => instance_Foldable_Data_Monoid_Dual_elem ;
+  fold := fun {m} `{GHC.Base.Monoid m} =>
     instance_Foldable_Data_Monoid_Dual_fold ;
-  foldMap := fun {m} {a} `{GHC.BaseGen.Monoid m} =>
+  foldMap := fun {m} {a} `{GHC.Base.Monoid m} =>
     instance_Foldable_Data_Monoid_Dual_foldMap ;
   foldl := fun {b} {a} => instance_Foldable_Data_Monoid_Dual_foldl ;
   foldl' := fun {b} {a} => instance_Foldable_Data_Monoid_Dual_foldl' ;
@@ -1353,9 +1351,9 @@ Instance instance_Foldable_Data_Monoid_Dual : !Foldable Data.Monoid.Dual := {
   foldr' := fun {a} {b} => instance_Foldable_Data_Monoid_Dual_foldr' ;
   foldr1 := fun {a} => instance_Foldable_Data_Monoid_Dual_foldr1 ;
   length := fun {a} => instance_Foldable_Data_Monoid_Dual_length ;
-  maximum := fun {a} `{GHC.Prim.Ord a} =>
+  maximum := fun {a} `{GHC.Base.Ord a} =>
     instance_Foldable_Data_Monoid_Dual_maximum ;
-  minimum := fun {a} `{GHC.Prim.Ord a} =>
+  minimum := fun {a} `{GHC.Base.Ord a} =>
     instance_Foldable_Data_Monoid_Dual_minimum ;
   null := fun {a} => instance_Foldable_Data_Monoid_Dual_null ;
   product := fun {a} `{GHC.Num.Num a} =>
@@ -1392,7 +1390,7 @@ Local Definition instance_Foldable__sum_a__foldr1 : forall {a}{a0},
                         match arg_36__ , arg_37__ with
                           | x , m => Some (match m with | None => x | (Some y) => f x y end)
                         end in
-                    Data.Maybe.fromMaybe (GHC.Prim.errorWithoutStackTrace
+                    Data.Maybe.fromMaybe (GHC.Base.errorWithoutStackTrace
                                          &"foldr1: empty structure") (instance_Foldable__sum_a__foldr mf None xs)
       end. *)
 
@@ -1401,7 +1399,7 @@ Local Definition instance_Foldable__sum_a__toList : forall {a}{b},
   fun {a}{b} =>
     fun arg_54__ =>
       match arg_54__ with
-        | t => Prim.build (fun _ arg_55__ arg_56__ =>
+        | t => Base.build (fun _ arg_55__ arg_56__ =>
                                 match arg_55__ , arg_56__ with
                                   | c , n => instance_Foldable__sum_a__foldr c n t
                                 end)
@@ -1415,17 +1413,17 @@ Local Definition instance_Foldable__sum_a__foldl' : forall{a0} {b} {a},
         | f , z0 , xs => let f' :=
                            fun arg_27__ arg_28__ arg_29__ =>
                              match arg_27__ , arg_28__ , arg_29__ with
-                               | x , k , z => GHC.BaseGen.op_zdzn__ k (f z x)
+                               | x , k , z => GHC.Base.op_zdzn__ k (f z x)
                              end in
-                         instance_Foldable__sum_a__foldr f' GHC.BaseGen.id xs z0
+                         instance_Foldable__sum_a__foldr f' GHC.Base.id xs z0
       end.
 
 Local Definition instance_Foldable__sum_a__foldMap : forall {a0}{m} {a},
-                                                       forall `{GHC.BaseGen.Monoid m}, (a -> m) -> (a + a0) -> m :=
-  fun {a0} {m} {a} `{GHC.BaseGen.Monoid m} =>
+                                                       forall `{GHC.Base.Monoid m}, (a -> m) -> (a + a0) -> m :=
+  fun {a0} {m} {a} `{GHC.Base.Monoid m} =>
     fun arg_295__ arg_296__ =>
       match arg_295__ , arg_296__ with
-        | _ , (inr _) => GHC.BaseGen.mempty
+        | _ , (inr _) => GHC.Base.mempty
         | f , (inl y) => f y
       end.
 
@@ -1437,7 +1435,7 @@ Local Definition instance_Foldable__sum_a__foldl : forall {a0} {b} {a},
       match arg_19__ , arg_20__ , arg_21__ with
         | f , z , t => Data.Monoid.appEndo (Data.Monoid.getDual (instance_Foldable__sum_a__foldMap
                                         (Coq.Program.Basics.compose Data.Monoid.Dual (Coq.Program.Basics.compose
-                                                                    Data.Monoid.Endo (GHC.BaseGen.flip f))) t)) z
+                                                                    Data.Monoid.Endo (GHC.Base.flip f))) t)) z
       end.
 
 Local Definition instance_Foldable__sum_a__foldl1 : forall {a},
@@ -1450,7 +1448,7 @@ Local Definition instance_Foldable__sum_a__foldl1 : forall {a},
                         match arg_46__ , arg_47__ with
                           | m , y => Some (match m with | None => y | (Some x) => f x y end)
                         end in
-                    Data.Maybe.fromMaybe (GHC.Prim.errorWithoutStackTrace
+                    Data.Maybe.fromMaybe (GHC.Base.errorWithoutStackTrace
                                          &"foldl1: empty structure") (instance_Foldable__sum_a__foldl mf None xs)
       end.
 *)
@@ -1463,9 +1461,9 @@ Local Definition instance_Foldable__sum_a__foldr' : forall {a0}{a} {b},
         | f , z0 , xs => let f' :=
                            fun arg_12__ arg_13__ arg_14__ =>
                              match arg_12__ , arg_13__ , arg_14__ with
-                               | k , x , z => GHC.BaseGen.op_zdzn__ k (f x z)
+                               | k , x , z => GHC.Base.op_zdzn__ k (f x z)
                              end in
-                         instance_Foldable__sum_a__foldl f' GHC.BaseGen.id xs z0
+                         instance_Foldable__sum_a__foldl f' GHC.Base.id xs z0
       end. *)
 
 Local Definition instance_Foldable__sum_a__product : forall {a}{a0},
@@ -1479,19 +1477,19 @@ Local Definition instance_Foldable__sum_a__sum : forall {a}{a0},
     Data.Monoid.getSum (instance_Foldable__sum_a__foldMap Data.Monoid.Mk_Sum x).
 
 Local Definition instance_Foldable__sum_a__fold : forall {a}{m},
-                                                    forall `{GHC.BaseGen.Monoid m}, (m + a) -> m :=
-  fun {a}{m} `{GHC.BaseGen.Monoid m} =>
-    instance_Foldable__sum_a__foldMap GHC.BaseGen.id.
+                                                    forall `{GHC.Base.Monoid m}, (m + a) -> m :=
+  fun {a}{m} `{GHC.Base.Monoid m} =>
+    instance_Foldable__sum_a__foldMap GHC.Base.id.
 
 (*
 Local Definition instance_Foldable__sum_a__elem : forall {a},
-                                                    forall `{GHC.Prim.Eq_ a}, a -> (sum a) a -> bool :=
-  fun {a} `{GHC.Prim.Eq_ a} => Coq.Program.Basics.compose any GHC.Prim.op_zeze__.
+                                                    forall `{GHC.Base.Eq_ a}, a -> (sum a) a -> bool :=
+  fun {a} `{GHC.Base.Eq_ a} => Coq.Program.Basics.compose any GHC.Base.op_zeze__.
 *)
 Instance instance_Foldable_list : !Foldable list := {
-  elem := fun {a} `{GHC.Prim.Eq_ a} => instance_Foldable_list_elem ;
-  fold := fun {m} `{GHC.BaseGen.Monoid m} => instance_Foldable_list_fold ;
-  foldMap := fun {m} {a} `{GHC.BaseGen.Monoid m} =>
+  elem := fun {a} `{GHC.Base.Eq_ a} => instance_Foldable_list_elem ;
+  fold := fun {m} `{GHC.Base.Monoid m} => instance_Foldable_list_fold ;
+  foldMap := fun {m} {a} `{GHC.Base.Monoid m} =>
     instance_Foldable_list_foldMap ;
   foldl := fun {b} {a} => instance_Foldable_list_foldl ;
   foldl' := fun {b} {a} => instance_Foldable_list_foldl' ;
@@ -1500,8 +1498,8 @@ Instance instance_Foldable_list : !Foldable list := {
   foldr' := fun {a} {b} => instance_Foldable_list_foldr' ;
   foldr1 := fun {a} => instance_Foldable_list_foldr1 ;
   length := fun {a} => instance_Foldable_list_length ;
-  maximum := fun {a} `{GHC.Prim.Ord a} => instance_Foldable_list_maximum ;
-  minimum := fun {a} `{GHC.Prim.Ord a} => instance_Foldable_list_minimum ;
+  maximum := fun {a} `{GHC.Base.Ord a} => instance_Foldable_list_maximum ;
+  minimum := fun {a} `{GHC.Base.Ord a} => instance_Foldable_list_minimum ;
   null := fun {a} => instance_Foldable_list_null ;
   product := fun {a} `{GHC.Num.Num a} => instance_Foldable_list_product ;
   sum := fun {a} `{GHC.Num.Num a} => instance_Foldable_list_sum ;
@@ -1512,7 +1510,7 @@ Definition concatMap {t} {a} {b} `{Foldable t} : (a -> list b) -> t a -> list
                                                  b :=
   fun arg_113__ arg_114__ =>
     match arg_113__ , arg_114__ with
-      | f , xs => Prim.build (fun _ arg_115__ arg_116__ =>
+      | f , xs => Base.build (fun _ arg_115__ arg_116__ =>
                                    match arg_115__ , arg_116__ with
                                      | c , n => foldr (fun arg_117__ arg_118__ =>
                                                         match arg_117__ , arg_118__ with
@@ -1524,7 +1522,7 @@ Definition concatMap {t} {a} {b} `{Foldable t} : (a -> list b) -> t a -> list
 Definition concat {t} {a} `{Foldable t} : t (list a) -> list a :=
   fun arg_125__ =>
     match arg_125__ with
-      | xs => Prim.build (fun _ arg_126__ arg_127__ =>
+      | xs => Base.build (fun _ arg_126__ arg_127__ =>
                                match arg_126__ , arg_127__ with
                                  | c , n => foldr (fun arg_128__ arg_129__ =>
                                                     match arg_128__ , arg_129__ with
@@ -1543,75 +1541,75 @@ Definition getMax {a} (arg_75__ : Max a) :=
 
 (*
 Local Definition instance_Foldable_GHC_Generics_U1_maximum : forall {a},
-                                                               forall `{GHC.Prim.Ord a}, GHC.Generics.U1 a -> a :=
-  fun {a} `{GHC.Prim.Ord a} =>
+                                                               forall `{GHC.Base.Ord a}, GHC.Generics.U1 a -> a :=
+  fun {a} `{GHC.Base.Ord a} =>
     Coq.Program.Basics.compose (Data.Maybe.fromMaybe
-                               (GHC.Prim.errorWithoutStackTrace &"maximum: empty structure"))
+                               (GHC.Base.errorWithoutStackTrace &"maximum: empty structure"))
                                (Coq.Program.Basics.compose getMax (instance_Foldable_GHC_Generics_U1_foldMap
                                                            (hashDot Mk_Max (Some : a -> option a)))).
 *)
 
-Instance instance_forall___GHC_Prim_Ord_a___GHC_BaseGen_Monoid__Max_a_
-  : !forall `{GHC.Prim.Ord a}, GHC.BaseGen.Monoid (Max a) := {}.
+Instance instance_forall___GHC_Base_Ord_a___GHC_Base_Monoid__Max_a_
+  : !forall `{GHC.Base.Ord a}, GHC.Base.Monoid (Max a) := {}.
 Proof.
 Admitted.
 
 (*
 Local Definition instance_Foldable_Data_Monoid_Last_maximum : forall {a},
-                                                                forall `{GHC.Prim.Ord a}, Data.Monoid.Last a -> a :=
-  fun {a} `{GHC.Prim.Ord a} =>
+                                                                forall `{GHC.Base.Ord a}, Data.Monoid.Last a -> a :=
+  fun {a} `{GHC.Base.Ord a} =>
     Coq.Program.Basics.compose (Data.Maybe.fromMaybe
-                               (GHC.Prim.errorWithoutStackTrace &"maximum: empty structure"))
+                               (GHC.Base.errorWithoutStackTrace &"maximum: empty structure"))
                                (Coq.Program.Basics.compose getMax (instance_Foldable_Data_Monoid_Last_foldMap
                                                            (hashDot Mk_Max (Some : a -> option a)))).
 
 Local Definition instance_Foldable_Data_Monoid_First_maximum : forall {a},
-                                                                 forall `{GHC.Prim.Ord a}, Data.Monoid.First a -> a :=
-  fun {a} `{GHC.Prim.Ord a} =>
+                                                                 forall `{GHC.Base.Ord a}, Data.Monoid.First a -> a :=
+  fun {a} `{GHC.Base.Ord a} =>
     Coq.Program.Basics.compose (Data.Maybe.fromMaybe
-                               (GHC.Prim.errorWithoutStackTrace &"maximum: empty structure"))
+                               (GHC.Base.errorWithoutStackTrace &"maximum: empty structure"))
                                (Coq.Program.Basics.compose getMax (instance_Foldable_Data_Monoid_First_foldMap
                                                            (hashDot Mk_Max (Some : a -> option a)))).
 
 Local Definition instance_Foldable_Data_Proxy_Proxy_maximum : forall {a},
-                                                                forall `{GHC.Prim.Ord a}, Data.Proxy.Proxy a -> a :=
-  fun {a} `{GHC.Prim.Ord a} =>
+                                                                forall `{GHC.Base.Ord a}, Data.Proxy.Proxy a -> a :=
+  fun {a} `{GHC.Base.Ord a} =>
     Coq.Program.Basics.compose (Data.Maybe.fromMaybe
-                               (GHC.Prim.errorWithoutStackTrace &"maximum: empty structure"))
+                               (GHC.Base.errorWithoutStackTrace &"maximum: empty structure"))
                                (Coq.Program.Basics.compose getMax (instance_Foldable_Data_Proxy_Proxy_foldMap
                                                            (hashDot Mk_Max (Some : a -> option a)))).
 
 Local Definition instance_Foldable__GHC_Arr_Array_i__maximum : forall {a},
-                                                                 forall `{GHC.Prim.Ord a}, (GHC.Arr.Array i) a -> a :=
-  fun {a} `{GHC.Prim.Ord a} =>
+                                                                 forall `{GHC.Base.Ord a}, (GHC.Arr.Array i) a -> a :=
+  fun {a} `{GHC.Base.Ord a} =>
     Coq.Program.Basics.compose (Data.Maybe.fromMaybe
-                               (GHC.Prim.errorWithoutStackTrace &"maximum: empty structure"))
+                               (GHC.Base.errorWithoutStackTrace &"maximum: empty structure"))
                                (Coq.Program.Basics.compose getMax (instance_Foldable__GHC_Arr_Array_i__foldMap
                                                            (hashDot Mk_Max (Some : a -> option a)))).
 
 Local Definition instance_Foldable__GHC_Tuple_____a__maximum : forall {a},
-                                                                 forall `{GHC.Prim.Ord a}, (GHC.Tuple.[,] a) a -> a :=
-  fun {a} `{GHC.Prim.Ord a} =>
+                                                                 forall `{GHC.Base.Ord a}, (GHC.Tuple.[,] a) a -> a :=
+  fun {a} `{GHC.Base.Ord a} =>
     Coq.Program.Basics.compose (Data.Maybe.fromMaybe
-                               (GHC.Prim.errorWithoutStackTrace &"maximum: empty structure"))
+                               (GHC.Base.errorWithoutStackTrace &"maximum: empty structure"))
                                (Coq.Program.Basics.compose getMax (instance_Foldable__GHC_Tuple_____a__foldMap
                                                            (hashDot Mk_Max (Some : a -> option a)))).
 
 Local Definition instance_Foldable__sum_a__maximum : forall {a},
-                                                       forall `{GHC.Prim.Ord a}, (sum a) a -> a :=
-  fun {a} `{GHC.Prim.Ord a} =>
+                                                       forall `{GHC.Base.Ord a}, (sum a) a -> a :=
+  fun {a} `{GHC.Base.Ord a} =>
     Coq.Program.Basics.compose (Data.Maybe.fromMaybe
-                               (GHC.Prim.errorWithoutStackTrace &"maximum: empty structure"))
+                               (GHC.Base.errorWithoutStackTrace &"maximum: empty structure"))
                                (Coq.Program.Basics.compose getMax (instance_Foldable__sum_a__foldMap (hashDot
                                                                                                      Mk_Max
                                                                                                      (Some : a -> option
                                                                                                      a)))).
 
 Local Definition instance_Foldable_option_maximum : forall {a},
-                                                      forall `{GHC.Prim.Ord a}, option a -> a :=
-  fun {a} `{GHC.Prim.Ord a} =>
+                                                      forall `{GHC.Base.Ord a}, option a -> a :=
+  fun {a} `{GHC.Base.Ord a} =>
     Coq.Program.Basics.compose (Data.Maybe.fromMaybe
-                               (GHC.Prim.errorWithoutStackTrace &"maximum: empty structure"))
+                               (GHC.Base.errorWithoutStackTrace &"maximum: empty structure"))
                                (Coq.Program.Basics.compose getMax (instance_Foldable_option_foldMap (hashDot
                                                                                                     Mk_Max
                                                                                                     (Some : a -> option
@@ -1625,18 +1623,18 @@ Definition getMin {a} (arg_74__ : Min a) :=
   end.
 
 Local Definition instance_Foldable_GHC_Generics_U1_minimum : forall {a},
-                                                               forall `{GHC.Prim.Ord a}, GHC.Generics.U1 a -> a :=
-  fun {a} `{GHC.Prim.Ord a} =>
+                                                               forall `{GHC.Base.Ord a}, GHC.Generics.U1 a -> a :=
+  fun {a} `{GHC.Base.Ord a} =>
     Coq.Program.Basics.compose (Data.Maybe.fromMaybe
-                               (GHC.Prim.errorWithoutStackTrace &"minimum: empty structure"))
+                               (GHC.Base.errorWithoutStackTrace &"minimum: empty structure"))
                                (Coq.Program.Basics.compose getMin (instance_Foldable_GHC_Generics_U1_foldMap
                                                            (hashDot Mk_Min (Some : a -> option a)))).
 
 Instance instance_Foldable_GHC_Generics_U1 : !Foldable GHC.Generics.U1 := {
-  elem := fun {a} `{GHC.Prim.Eq_ a} => instance_Foldable_GHC_Generics_U1_elem ;
-  fold := fun {m} `{GHC.BaseGen.Monoid m} =>
+  elem := fun {a} `{GHC.Base.Eq_ a} => instance_Foldable_GHC_Generics_U1_elem ;
+  fold := fun {m} `{GHC.Base.Monoid m} =>
     instance_Foldable_GHC_Generics_U1_fold ;
-  foldMap := fun {m} {a} `{GHC.BaseGen.Monoid m} =>
+  foldMap := fun {m} {a} `{GHC.Base.Monoid m} =>
     instance_Foldable_GHC_Generics_U1_foldMap ;
   foldl := fun {b} {a} => instance_Foldable_GHC_Generics_U1_foldl ;
   foldl' := fun {b} {a} => instance_Foldable_GHC_Generics_U1_foldl' ;
@@ -1645,9 +1643,9 @@ Instance instance_Foldable_GHC_Generics_U1 : !Foldable GHC.Generics.U1 := {
   foldr' := fun {a} {b} => instance_Foldable_GHC_Generics_U1_foldr' ;
   foldr1 := fun {a} => instance_Foldable_GHC_Generics_U1_foldr1 ;
   length := fun {a} => instance_Foldable_GHC_Generics_U1_length ;
-  maximum := fun {a} `{GHC.Prim.Ord a} =>
+  maximum := fun {a} `{GHC.Base.Ord a} =>
     instance_Foldable_GHC_Generics_U1_maximum ;
-  minimum := fun {a} `{GHC.Prim.Ord a} =>
+  minimum := fun {a} `{GHC.Base.Ord a} =>
     instance_Foldable_GHC_Generics_U1_minimum ;
   null := fun {a} => instance_Foldable_GHC_Generics_U1_null ;
   product := fun {a} `{GHC.Num.Num a} =>
@@ -1656,27 +1654,27 @@ Instance instance_Foldable_GHC_Generics_U1 : !Foldable GHC.Generics.U1 := {
   toList := fun {a} => instance_Foldable_GHC_Generics_U1_toList }.
 *)
 
-Instance instance_forall___GHC_Prim_Ord_a___GHC_BaseGen_Monoid__Min_a_
-  : !forall `{GHC.Prim.Ord a}, GHC.BaseGen.Monoid (Min a) := {}.
+Instance instance_forall___GHC_Base_Ord_a___GHC_Base_Monoid__Min_a_
+  : !forall `{GHC.Base.Ord a}, GHC.Base.Monoid (Min a) := {}.
 Proof.
 Admitted.
 
 (*
 Local Definition instance_Foldable_Data_Monoid_Last_minimum : forall {a},
-                                                                forall `{GHC.Prim.Ord a}, Data.Monoid.Last a -> a :=
-  fun {a} `{GHC.Prim.Ord a} =>
+                                                                forall `{GHC.Base.Ord a}, Data.Monoid.Last a -> a :=
+  fun {a} `{GHC.Base.Ord a} =>
     Coq.Program.Basics.compose (Data.Maybe.fromMaybe
-                               (GHC.Prim.errorWithoutStackTrace &"minimum: empty structure"))
+                               (GHC.Base.errorWithoutStackTrace &"minimum: empty structure"))
                                (Coq.Program.Basics.compose getMin (instance_Foldable_Data_Monoid_Last_foldMap
                                                            (hashDot Mk_Min (Some : a -> option a)))).
 *)
 
 (*
 Instance instance_Foldable_Data_Monoid_Last : !Foldable Data.Monoid.Last := {
-  elem := fun {a} `{GHC.Prim.Eq_ a} => instance_Foldable_Data_Monoid_Last_elem ;
-  fold := fun {m} `{GHC.BaseGen.Monoid m} =>
+  elem := fun {a} `{GHC.Base.Eq_ a} => instance_Foldable_Data_Monoid_Last_elem ;
+  fold := fun {m} `{GHC.Base.Monoid m} =>
     instance_Foldable_Data_Monoid_Last_fold ;
-  foldMap := fun {m} {a} `{GHC.BaseGen.Monoid m} =>
+  foldMap := fun {m} {a} `{GHC.Base.Monoid m} =>
     instance_Foldable_Data_Monoid_Last_foldMap ;
   foldl := fun {b} {a} => instance_Foldable_Data_Monoid_Last_foldl ;
   foldl' := fun {b} {a} => instance_Foldable_Data_Monoid_Last_foldl' ;
@@ -1685,9 +1683,9 @@ Instance instance_Foldable_Data_Monoid_Last : !Foldable Data.Monoid.Last := {
   foldr' := fun {a} {b} => instance_Foldable_Data_Monoid_Last_foldr' ;
   foldr1 := fun {a} => instance_Foldable_Data_Monoid_Last_foldr1 ;
   length := fun {a} => instance_Foldable_Data_Monoid_Last_length ;
-  maximum := fun {a} `{GHC.Prim.Ord a} =>
+  maximum := fun {a} `{GHC.Base.Ord a} =>
     instance_Foldable_Data_Monoid_Last_maximum ;
-  minimum := fun {a} `{GHC.Prim.Ord a} =>
+  minimum := fun {a} `{GHC.Base.Ord a} =>
     instance_Foldable_Data_Monoid_Last_minimum ;
   null := fun {a} => instance_Foldable_Data_Monoid_Last_null ;
   product := fun {a} `{GHC.Num.Num a} =>
@@ -1696,18 +1694,18 @@ Instance instance_Foldable_Data_Monoid_Last : !Foldable Data.Monoid.Last := {
   toList := fun {a} => instance_Foldable_Data_Monoid_Last_toList }.
 
 Local Definition instance_Foldable_Data_Monoid_First_minimum : forall {a},
-                                                                 forall `{GHC.Prim.Ord a}, Data.Monoid.First a -> a :=
-  fun {a} `{GHC.Prim.Ord a} =>
+                                                                 forall `{GHC.Base.Ord a}, Data.Monoid.First a -> a :=
+  fun {a} `{GHC.Base.Ord a} =>
     Coq.Program.Basics.compose (Data.Maybe.fromMaybe
-                               (GHC.Prim.errorWithoutStackTrace &"minimum: empty structure"))
+                               (GHC.Base.errorWithoutStackTrace &"minimum: empty structure"))
                                (Coq.Program.Basics.compose getMin (instance_Foldable_Data_Monoid_First_foldMap
                                                            (hashDot Mk_Min (Some : a -> option a)))).
 
 Instance instance_Foldable_Data_Monoid_First : !Foldable Data.Monoid.First := {
-  elem := fun {a} `{GHC.Prim.Eq_ a} => instance_Foldable_Data_Monoid_First_elem ;
-  fold := fun {m} `{GHC.BaseGen.Monoid m} =>
+  elem := fun {a} `{GHC.Base.Eq_ a} => instance_Foldable_Data_Monoid_First_elem ;
+  fold := fun {m} `{GHC.Base.Monoid m} =>
     instance_Foldable_Data_Monoid_First_fold ;
-  foldMap := fun {m} {a} `{GHC.BaseGen.Monoid m} =>
+  foldMap := fun {m} {a} `{GHC.Base.Monoid m} =>
     instance_Foldable_Data_Monoid_First_foldMap ;
   foldl := fun {b} {a} => instance_Foldable_Data_Monoid_First_foldl ;
   foldl' := fun {b} {a} => instance_Foldable_Data_Monoid_First_foldl' ;
@@ -1716,9 +1714,9 @@ Instance instance_Foldable_Data_Monoid_First : !Foldable Data.Monoid.First := {
   foldr' := fun {a} {b} => instance_Foldable_Data_Monoid_First_foldr' ;
   foldr1 := fun {a} => instance_Foldable_Data_Monoid_First_foldr1 ;
   length := fun {a} => instance_Foldable_Data_Monoid_First_length ;
-  maximum := fun {a} `{GHC.Prim.Ord a} =>
+  maximum := fun {a} `{GHC.Base.Ord a} =>
     instance_Foldable_Data_Monoid_First_maximum ;
-  minimum := fun {a} `{GHC.Prim.Ord a} =>
+  minimum := fun {a} `{GHC.Base.Ord a} =>
     instance_Foldable_Data_Monoid_First_minimum ;
   null := fun {a} => instance_Foldable_Data_Monoid_First_null ;
   product := fun {a} `{GHC.Num.Num a} =>
@@ -1728,20 +1726,20 @@ Instance instance_Foldable_Data_Monoid_First : !Foldable Data.Monoid.First := {
 *)
 (*
 Local Definition instance_Foldable_Data_Proxy_Proxy_minimum : forall {a},
-                                                                forall `{GHC.Prim.Ord a}, Data.Proxy.Proxy a -> a :=
-  fun {a} `{GHC.Prim.Ord a} =>
+                                                                forall `{GHC.Base.Ord a}, Data.Proxy.Proxy a -> a :=
+  fun {a} `{GHC.Base.Ord a} =>
     Coq.Program.Basics.compose (Data.Maybe.fromMaybe
-                               (GHC.Prim.errorWithoutStackTrace &"minimum: empty structure"))
+                               (GHC.Base.errorWithoutStackTrace &"minimum: empty structure"))
                                (Coq.Program.Basics.compose getMin (instance_Foldable_Data_Proxy_Proxy_foldMap
                                                            (hashDot Mk_Min (Some : a -> option a)))).
 *)
 
 (*
 Instance instance_Foldable_Data_Proxy_Proxy : !Foldable Data.Proxy.Proxy := {
-  elem := fun {a} `{GHC.Prim.Eq_ a} => instance_Foldable_Data_Proxy_Proxy_elem ;
-  fold := fun {m} `{GHC.BaseGen.Monoid m} =>
+  elem := fun {a} `{GHC.Base.Eq_ a} => instance_Foldable_Data_Proxy_Proxy_elem ;
+  fold := fun {m} `{GHC.Base.Monoid m} =>
     instance_Foldable_Data_Proxy_Proxy_fold ;
-  foldMap := fun {m} {a} `{GHC.BaseGen.Monoid m} =>
+  foldMap := fun {m} {a} `{GHC.Base.Monoid m} =>
     instance_Foldable_Data_Proxy_Proxy_foldMap ;
   foldl := fun {b} {a} => instance_Foldable_Data_Proxy_Proxy_foldl ;
   foldl' := fun {b} {a} => instance_Foldable_Data_Proxy_Proxy_foldl' ;
@@ -1750,9 +1748,9 @@ Instance instance_Foldable_Data_Proxy_Proxy : !Foldable Data.Proxy.Proxy := {
   foldr' := fun {a} {b} => instance_Foldable_Data_Proxy_Proxy_foldr' ;
   foldr1 := fun {a} => instance_Foldable_Data_Proxy_Proxy_foldr1 ;
   length := fun {a} => instance_Foldable_Data_Proxy_Proxy_length ;
-  maximum := fun {a} `{GHC.Prim.Ord a} =>
+  maximum := fun {a} `{GHC.Base.Ord a} =>
     instance_Foldable_Data_Proxy_Proxy_maximum ;
-  minimum := fun {a} `{GHC.Prim.Ord a} =>
+  minimum := fun {a} `{GHC.Base.Ord a} =>
     instance_Foldable_Data_Proxy_Proxy_minimum ;
   null := fun {a} => instance_Foldable_Data_Proxy_Proxy_null ;
   product := fun {a} `{GHC.Num.Num a} =>
@@ -1763,18 +1761,18 @@ Instance instance_Foldable_Data_Proxy_Proxy : !Foldable Data.Proxy.Proxy := {
 
 (*
 Local Definition instance_Foldable__GHC_Arr_Array_i__minimum : forall {a},
-                                                                 forall `{GHC.Prim.Ord a}, (GHC.Arr.Array i) a -> a :=
-  fun {a} `{GHC.Prim.Ord a} =>
+                                                                 forall `{GHC.Base.Ord a}, (GHC.Arr.Array i) a -> a :=
+  fun {a} `{GHC.Base.Ord a} =>
     Coq.Program.Basics.compose (Data.Maybe.fromMaybe
-                               (GHC.Prim.errorWithoutStackTrace &"minimum: empty structure"))
+                               (GHC.Base.errorWithoutStackTrace &"minimum: empty structure"))
                                (Coq.Program.Basics.compose getMin (instance_Foldable__GHC_Arr_Array_i__foldMap
                                                            (hashDot Mk_Min (Some : a -> option a)))).
 
 Instance instance_Foldable__GHC_Arr_Array_i_ : !Foldable (GHC.Arr.Array i) := {
-  elem := fun {a} `{GHC.Prim.Eq_ a} => instance_Foldable__GHC_Arr_Array_i__elem ;
-  fold := fun {m} `{GHC.BaseGen.Monoid m} =>
+  elem := fun {a} `{GHC.Base.Eq_ a} => instance_Foldable__GHC_Arr_Array_i__elem ;
+  fold := fun {m} `{GHC.Base.Monoid m} =>
     instance_Foldable__GHC_Arr_Array_i__fold ;
-  foldMap := fun {m} {a} `{GHC.BaseGen.Monoid m} =>
+  foldMap := fun {m} {a} `{GHC.Base.Monoid m} =>
     instance_Foldable__GHC_Arr_Array_i__foldMap ;
   foldl := fun {b} {a} => instance_Foldable__GHC_Arr_Array_i__foldl ;
   foldl' := fun {b} {a} => instance_Foldable__GHC_Arr_Array_i__foldl' ;
@@ -1783,9 +1781,9 @@ Instance instance_Foldable__GHC_Arr_Array_i_ : !Foldable (GHC.Arr.Array i) := {
   foldr' := fun {a} {b} => instance_Foldable__GHC_Arr_Array_i__foldr' ;
   foldr1 := fun {a} => instance_Foldable__GHC_Arr_Array_i__foldr1 ;
   length := fun {a} => instance_Foldable__GHC_Arr_Array_i__length ;
-  maximum := fun {a} `{GHC.Prim.Ord a} =>
+  maximum := fun {a} `{GHC.Base.Ord a} =>
     instance_Foldable__GHC_Arr_Array_i__maximum ;
-  minimum := fun {a} `{GHC.Prim.Ord a} =>
+  minimum := fun {a} `{GHC.Base.Ord a} =>
     instance_Foldable__GHC_Arr_Array_i__minimum ;
   null := fun {a} => instance_Foldable__GHC_Arr_Array_i__null ;
   product := fun {a} `{GHC.Num.Num a} =>
@@ -1794,18 +1792,18 @@ Instance instance_Foldable__GHC_Arr_Array_i_ : !Foldable (GHC.Arr.Array i) := {
   toList := fun {a} => instance_Foldable__GHC_Arr_Array_i__toList }.
 
 Local Definition instance_Foldable__GHC_Tuple_____a__minimum : forall {a},
-                                                                 forall `{GHC.Prim.Ord a}, (GHC.Tuple.[,] a) a -> a :=
-  fun {a} `{GHC.Prim.Ord a} =>
+                                                                 forall `{GHC.Base.Ord a}, (GHC.Tuple.[,] a) a -> a :=
+  fun {a} `{GHC.Base.Ord a} =>
     Coq.Program.Basics.compose (Data.Maybe.fromMaybe
-                               (GHC.Prim.errorWithoutStackTrace &"minimum: empty structure"))
+                               (GHC.Base.errorWithoutStackTrace &"minimum: empty structure"))
                                (Coq.Program.Basics.compose getMin (instance_Foldable__GHC_Tuple_____a__foldMap
                                                            (hashDot Mk_Min (Some : a -> option a)))).
 
 Instance instance_Foldable__GHC_Tuple_____a_ : !Foldable (GHC.Tuple.[,] a) := {
-  elem := fun {a} `{GHC.Prim.Eq_ a} => instance_Foldable__GHC_Tuple_____a__elem ;
-  fold := fun {m} `{GHC.BaseGen.Monoid m} =>
+  elem := fun {a} `{GHC.Base.Eq_ a} => instance_Foldable__GHC_Tuple_____a__elem ;
+  fold := fun {m} `{GHC.Base.Monoid m} =>
     instance_Foldable__GHC_Tuple_____a__fold ;
-  foldMap := fun {m} {a} `{GHC.BaseGen.Monoid m} =>
+  foldMap := fun {m} {a} `{GHC.Base.Monoid m} =>
     instance_Foldable__GHC_Tuple_____a__foldMap ;
   foldl := fun {b} {a} => instance_Foldable__GHC_Tuple_____a__foldl ;
   foldl' := fun {b} {a} => instance_Foldable__GHC_Tuple_____a__foldl' ;
@@ -1814,9 +1812,9 @@ Instance instance_Foldable__GHC_Tuple_____a_ : !Foldable (GHC.Tuple.[,] a) := {
   foldr' := fun {a} {b} => instance_Foldable__GHC_Tuple_____a__foldr' ;
   foldr1 := fun {a} => instance_Foldable__GHC_Tuple_____a__foldr1 ;
   length := fun {a} => instance_Foldable__GHC_Tuple_____a__length ;
-  maximum := fun {a} `{GHC.Prim.Ord a} =>
+  maximum := fun {a} `{GHC.Base.Ord a} =>
     instance_Foldable__GHC_Tuple_____a__maximum ;
-  minimum := fun {a} `{GHC.Prim.Ord a} =>
+  minimum := fun {a} `{GHC.Base.Ord a} =>
     instance_Foldable__GHC_Tuple_____a__minimum ;
   null := fun {a} => instance_Foldable__GHC_Tuple_____a__null ;
   product := fun {a} `{GHC.Num.Num a} =>
@@ -1826,10 +1824,10 @@ Instance instance_Foldable__GHC_Tuple_____a_ : !Foldable (GHC.Tuple.[,] a) := {
 *)
 (*
 Local Definition instance_Foldable__sum_a__minimum : forall {a},
-                                                       forall `{GHC.Prim.Ord a}, (sum a) a -> a :=
-  fun {a} `{GHC.Prim.Ord a} =>
+                                                       forall `{GHC.Base.Ord a}, (sum a) a -> a :=
+  fun {a} `{GHC.Base.Ord a} =>
     Coq.Program.Basics.compose (Data.Maybe.fromMaybe
-                               (GHC.Prim.errorWithoutStackTrace &"minimum: empty structure"))
+                               (GHC.Base.errorWithoutStackTrace &"minimum: empty structure"))
                                (Coq.Program.Basics.compose getMin (instance_Foldable__sum_a__foldMap (hashDot
                                                                                                      Mk_Min
                                                                                                      (Some : a -> option
@@ -1837,9 +1835,9 @@ Local Definition instance_Foldable__sum_a__minimum : forall {a},
 *)
 (*
 Instance instance_Foldable__sum_a_ : !Foldable (fun x => (a + x)%type) := {
-  elem := fun {a} `{GHC.Prim.Eq_ a} => instance_Foldable__sum_a__elem ;
-  fold := fun {m} `{GHC.BaseGen.Monoid m} => instance_Foldable__sum_a__fold ;
-  foldMap := fun {m} {a} `{GHC.BaseGen.Monoid m} =>
+  elem := fun {a} `{GHC.Base.Eq_ a} => instance_Foldable__sum_a__elem ;
+  fold := fun {m} `{GHC.Base.Monoid m} => instance_Foldable__sum_a__fold ;
+  foldMap := fun {m} {a} `{GHC.Base.Monoid m} =>
     instance_Foldable__sum_a__foldMap ;
   foldl := fun {b} {a} => instance_Foldable__sum_a__foldl ;
   foldl' := fun {b} {a} => instance_Foldable__sum_a__foldl' ;
@@ -1848,8 +1846,8 @@ Instance instance_Foldable__sum_a_ : !Foldable (fun x => (a + x)%type) := {
   foldr' := fun {a} {b} => instance_Foldable__sum_a__foldr' ;
   foldr1 := fun {a} => instance_Foldable__sum_a__foldr1 ;
   length := fun {a} => instance_Foldable__sum_a__length ;
-  maximum := fun {a} `{GHC.Prim.Ord a} => instance_Foldable__sum_a__maximum ;
-  minimum := fun {a} `{GHC.Prim.Ord a} => instance_Foldable__sum_a__minimum ;
+  maximum := fun {a} `{GHC.Base.Ord a} => instance_Foldable__sum_a__maximum ;
+  minimum := fun {a} `{GHC.Base.Ord a} => instance_Foldable__sum_a__minimum ;
   null := fun {a} => instance_Foldable__sum_a__null ;
   product := fun {a} `{GHC.Num.Num a} => instance_Foldable__sum_a__product ;
   sum := fun {a} `{GHC.Num.Num a} => instance_Foldable__sum_a__sum ;
@@ -1857,10 +1855,10 @@ Instance instance_Foldable__sum_a_ : !Foldable (fun x => (a + x)%type) := {
 *)
 (*
 Local Definition instance_Foldable_option_minimum : forall {a},
-                                                      forall `{GHC.Prim.Ord a}, option a -> a :=
-  fun {a} `{GHC.Prim.Ord a} =>
+                                                      forall `{GHC.Base.Ord a}, option a -> a :=
+  fun {a} `{GHC.Base.Ord a} =>
     Coq.Program.Basics.compose (Data.Maybe.fromMaybe
-                               (GHC.Prim.errorWithoutStackTrace &"minimum: empty structure"))
+                               (GHC.Base.errorWithoutStackTrace &"minimum: empty structure"))
                                (Coq.Program.Basics.compose getMin (instance_Foldable_option_foldMap (hashDot
                                                                                                     Mk_Min
                                                                                                     (Some : a -> option
@@ -1868,9 +1866,9 @@ Local Definition instance_Foldable_option_minimum : forall {a},
 *)
 (*
 Instance instance_Foldable_option : !Foldable option := {
-  elem := fun {a} `{GHC.Prim.Eq_ a} => instance_Foldable_option_elem ;
-  fold := fun {m} `{GHC.BaseGen.Monoid m} => instance_Foldable_option_fold ;
-  foldMap := fun {m} {a} `{GHC.BaseGen.Monoid m} =>
+  elem := fun {a} `{GHC.Base.Eq_ a} => instance_Foldable_option_elem ;
+  fold := fun {m} `{GHC.Base.Monoid m} => instance_Foldable_option_fold ;
+  foldMap := fun {m} {a} `{GHC.Base.Monoid m} =>
     instance_Foldable_option_foldMap ;
   foldl := fun {b} {a} => instance_Foldable_option_foldl ;
   foldl' := fun {b} {a} => instance_Foldable_option_foldl' ;
@@ -1879,8 +1877,8 @@ Instance instance_Foldable_option : !Foldable option := {
   foldr' := fun {a} {b} => instance_Foldable_option_foldr' ;
   foldr1 := fun {a} => instance_Foldable_option_foldr1 ;
   length := fun {a} => instance_Foldable_option_length ;
-  maximum := fun {a} `{GHC.Prim.Ord a} => instance_Foldable_option_maximum ;
-  minimum := fun {a} `{GHC.Prim.Ord a} => instance_Foldable_option_minimum ;
+  maximum := fun {a} `{GHC.Base.Ord a} => instance_Foldable_option_maximum ;
+  minimum := fun {a} `{GHC.Base.Ord a} => instance_Foldable_option_minimum ;
   null := fun {a} => instance_Foldable_option_null ;
   product := fun {a} `{GHC.Num.Num a} => instance_Foldable_option_product ;
   sum := fun {a} `{GHC.Num.Num a} => instance_Foldable_option_sum ;
@@ -1892,16 +1890,16 @@ Instance instance_Foldable_option : !Foldable option := {
      Data.Monoid.First Data.Monoid.Last Data.Monoid.Product Data.Monoid.Sum
      Data.Proxy.Proxy GHC.Arr.Array GHC.Arr.elems GHC.Arr.foldl1Elems
      GHC.Arr.foldlElems GHC.Arr.foldlElems' GHC.Arr.foldr1Elems GHC.Arr.foldrElems
-     GHC.Arr.foldrElems' GHC.Arr.numElements GHC.Base.MonadPlus Prim.build
+     GHC.Arr.foldrElems' GHC.Arr.numElements GHC.Base.MonadPlus Base.build
      GHC.Base.empty GHC.Base.mappend GHC.Base.mempty GHC.Base.op_zdzn__
      GHC.Base.op_zgzg__ GHC.Base.op_zgzgze__ GHC.Base.op_zlzbzg__ GHC.Base.op_ztzg__
-     GHC.Base.pure GHC.Base.return_ GHC.BaseGen.Alternative GHC.BaseGen.Applicative
-     GHC.BaseGen.Monad GHC.BaseGen.Monoid GHC.BaseGen.flip GHC.BaseGen.foldr
-     GHC.BaseGen.id GHC.Generics.U1 GHC.List.elem GHC.List.foldl GHC.List.foldl'
+     GHC.Base.pure GHC.Base.return_ GHC.Base.Alternative GHC.Base.Applicative
+     GHC.Base.Monad GHC.Base.Monoid GHC.Base.flip GHC.Base.foldr
+     GHC.Base.id GHC.Generics.U1 GHC.List.elem GHC.List.foldl GHC.List.foldl'
      GHC.List.foldl1 GHC.List.foldr1 GHC.List.length GHC.List.maximum
      GHC.List.minimum GHC.List.null GHC.List.product GHC.List.sum GHC.Num.Int
-     GHC.Num.Num GHC.Num.op_zp__ GHC.Prim.Eq_ GHC.Prim.Ord GHC.Prim.coerce
-     GHC.Prim.errorWithoutStackTrace GHC.Prim.op_zeze__ GHC.Tuple.[,]
+     GHC.Num.Num GHC.Num.op_zp__ GHC.Base.Eq_ GHC.Base.Ord GHC.Base.coerce
+     GHC.Base.errorWithoutStackTrace GHC.Base.op_zeze__ GHC.Tuple.[,]
      GHC.Types.Coercible None Some appEndo bool comparison cons false getAll getAny
      getDual getFirst getLast getProduct getSum hashDot i inl inr list negb nil
      option pair true tt unit
