hs-to-coq/examples/ghc-base/lib/Data/Functor.v
@@ -13,29 +13,27 @@ Unset Printing Implicit Defensive.
 (* Converted imports: *)
 
 Require GHC.Base.
-Require GHC.BaseGen.
 
 (* Converted declarations: *)
 
-Definition op_zdzg__ {f} {a} {b} `{GHC.BaseGen.Functor f} : f a -> b -> f b :=
-  GHC.BaseGen.flip GHC.BaseGen.op_zlzd__.
+Definition op_zdzg__ {f} {a} {b} `{GHC.Base.Functor f} : f a -> b -> f b :=
+  GHC.Base.flip GHC.Base.op_zlzd__.
 
 Infix "$>" := (op_zdzg__) (at level 99).
 
 Notation "'_$>_'" := (op_zdzg__).
 
-Definition op_zlzdzg__ {f} {a} {b} `{GHC.BaseGen.Functor f} : (a -> b) -> f
-                                                              a -> f b :=
-  GHC.BaseGen.fmap.
+Definition op_zlzdzg__ {f} {a} {b} `{GHC.Base.Functor f} : (a -> b) -> f a -> f
+                                                           b :=
+  GHC.Base.fmap.
 
 Infix "<$>" := (op_zlzdzg__) (at level 99).
 
 Notation "'_<$>_'" := (op_zlzdzg__).
 
-Definition void {f} {a} `{GHC.BaseGen.Functor f} : f a -> f unit :=
-  fun arg_0__ => match arg_0__ with | x => GHC.BaseGen.op_zlzd__ tt x end.
+Definition void {f} {a} `{GHC.Base.Functor f} : f a -> f unit :=
+  fun arg_0__ => match arg_0__ with | x => GHC.Base.op_zlzd__ tt x end.
 
 (* Unbound variables:
-     GHC.BaseGen.Functor GHC.BaseGen.flip GHC.BaseGen.fmap GHC.BaseGen.op_zlzd__ tt
-     unit
+     GHC.Base.Functor GHC.Base.flip GHC.Base.fmap GHC.Base.op_zlzd__ tt unit
 *)
