hs-to-coq/examples/ghc-base/module-edits/GHC/Base/preamble.v
@@ -1,1 +1,1 @@
-Require Export Prim.
+(* Require Export Prim. *)
